feat: new smith models for searchable encryption

DynamoDbEncryptionMiddlewareInternal/runtimes/java/src/main/smithy-generated/software/amazon/cryptography/dynamoDbEncryption/ToDafny.java
@@ -15,10 +15,22 @@ import Dafny.Aws.Cryptography.DynamoDbEncryption.Types.BatchWriteItemInputTransf
 import Dafny.Aws.Cryptography.DynamoDbEncryption.Types.BatchWriteItemInputTransformOutput;
 import Dafny.Aws.Cryptography.DynamoDbEncryption.Types.BatchWriteItemOutputTransformInput;
 import Dafny.Aws.Cryptography.DynamoDbEncryption.Types.BatchWriteItemOutputTransformOutput;
+import Dafny.Aws.Cryptography.DynamoDbEncryption.Types.BeaconVersion;
+import Dafny.Aws.Cryptography.DynamoDbEncryption.Types.CompoundBeacon;
+import Dafny.Aws.Cryptography.DynamoDbEncryption.Types.Constructor;
+import Dafny.Aws.Cryptography.DynamoDbEncryption.Types.ConstructorPart;
+import Dafny.Aws.Cryptography.DynamoDbEncryption.Types.CreateTableInputTransformInput;
+import Dafny.Aws.Cryptography.DynamoDbEncryption.Types.CreateTableInputTransformOutput;
+import Dafny.Aws.Cryptography.DynamoDbEncryption.Types.CreateTableOutputTransformInput;
+import Dafny.Aws.Cryptography.DynamoDbEncryption.Types.CreateTableOutputTransformOutput;
 import Dafny.Aws.Cryptography.DynamoDbEncryption.Types.DeleteItemInputTransformInput;
 import Dafny.Aws.Cryptography.DynamoDbEncryption.Types.DeleteItemInputTransformOutput;
 import Dafny.Aws.Cryptography.DynamoDbEncryption.Types.DeleteItemOutputTransformInput;
 import Dafny.Aws.Cryptography.DynamoDbEncryption.Types.DeleteItemOutputTransformOutput;
+import Dafny.Aws.Cryptography.DynamoDbEncryption.Types.DescribeTableInputTransformInput;
+import Dafny.Aws.Cryptography.DynamoDbEncryption.Types.DescribeTableInputTransformOutput;
+import Dafny.Aws.Cryptography.DynamoDbEncryption.Types.DescribeTableOutputTransformInput;
+import Dafny.Aws.Cryptography.DynamoDbEncryption.Types.DescribeTableOutputTransformOutput;
 import Dafny.Aws.Cryptography.DynamoDbEncryption.Types.DynamoDbEncryptionConfig;
 import Dafny.Aws.Cryptography.DynamoDbEncryption.Types.DynamoDbTableEncryptionConfig;
 import Dafny.Aws.Cryptography.DynamoDbEncryption.Types.Error;
@@ -35,6 +47,7 @@ import Dafny.Aws.Cryptography.DynamoDbEncryption.Types.GetItemInputTransformInpu
 import Dafny.Aws.Cryptography.DynamoDbEncryption.Types.GetItemInputTransformOutput;
 import Dafny.Aws.Cryptography.DynamoDbEncryption.Types.GetItemOutputTransformInput;
 import Dafny.Aws.Cryptography.DynamoDbEncryption.Types.GetItemOutputTransformOutput;
+import Dafny.Aws.Cryptography.DynamoDbEncryption.Types.NonSensitivePart;
 import Dafny.Aws.Cryptography.DynamoDbEncryption.Types.PutItemInputTransformInput;
 import Dafny.Aws.Cryptography.DynamoDbEncryption.Types.PutItemInputTransformOutput;
 import Dafny.Aws.Cryptography.DynamoDbEncryption.Types.PutItemOutputTransformInput;
@@ -47,6 +60,9 @@ import Dafny.Aws.Cryptography.DynamoDbEncryption.Types.ScanInputTransformInput;
 import Dafny.Aws.Cryptography.DynamoDbEncryption.Types.ScanInputTransformOutput;
 import Dafny.Aws.Cryptography.DynamoDbEncryption.Types.ScanOutputTransformInput;
 import Dafny.Aws.Cryptography.DynamoDbEncryption.Types.ScanOutputTransformOutput;
+import Dafny.Aws.Cryptography.DynamoDbEncryption.Types.SearchConfig;
+import Dafny.Aws.Cryptography.DynamoDbEncryption.Types.SensitivePart;
+import Dafny.Aws.Cryptography.DynamoDbEncryption.Types.StandardBeacon;
 import Dafny.Aws.Cryptography.DynamoDbEncryption.Types.TransactGetItemsInputTransformInput;
 import Dafny.Aws.Cryptography.DynamoDbEncryption.Types.TransactGetItemsInputTransformOutput;
 import Dafny.Aws.Cryptography.DynamoDbEncryption.Types.TransactGetItemsOutputTransformInput;
@@ -59,6 +75,11 @@ import Dafny.Aws.Cryptography.DynamoDbEncryption.Types.UpdateItemInputTransformI
 import Dafny.Aws.Cryptography.DynamoDbEncryption.Types.UpdateItemInputTransformOutput;
 import Dafny.Aws.Cryptography.DynamoDbEncryption.Types.UpdateItemOutputTransformInput;
 import Dafny.Aws.Cryptography.DynamoDbEncryption.Types.UpdateItemOutputTransformOutput;
+import Dafny.Aws.Cryptography.DynamoDbEncryption.Types.UpdateTableInputTransformInput;
+import Dafny.Aws.Cryptography.DynamoDbEncryption.Types.UpdateTableInputTransformOutput;
+import Dafny.Aws.Cryptography.DynamoDbEncryption.Types.UpdateTableOutputTransformInput;
+import Dafny.Aws.Cryptography.DynamoDbEncryption.Types.UpdateTableOutputTransformOutput;
+import Dafny.Aws.Cryptography.DynamoDbEncryption.Types.VirtualField;
 import Dafny.Aws.Cryptography.MaterialProviders.Types.DBEAlgorithmSuiteId;
 import Dafny.Aws.Cryptography.MaterialProviders.Types.ICryptographicMaterialsManager;
 import Dafny.Aws.Cryptography.MaterialProviders.Types.IKeyring;
@@ -69,8 +90,12 @@ import Dafny.Com.Amazonaws.Dynamodb.Types.BatchGetItemInput;
 import Dafny.Com.Amazonaws.Dynamodb.Types.BatchGetItemOutput;
 import Dafny.Com.Amazonaws.Dynamodb.Types.BatchWriteItemInput;
 import Dafny.Com.Amazonaws.Dynamodb.Types.BatchWriteItemOutput;
+import Dafny.Com.Amazonaws.Dynamodb.Types.CreateTableInput;
+import Dafny.Com.Amazonaws.Dynamodb.Types.CreateTableOutput;
 import Dafny.Com.Amazonaws.Dynamodb.Types.DeleteItemInput;
 import Dafny.Com.Amazonaws.Dynamodb.Types.DeleteItemOutput;
+import Dafny.Com.Amazonaws.Dynamodb.Types.DescribeTableInput;
+import Dafny.Com.Amazonaws.Dynamodb.Types.DescribeTableOutput;
 import Dafny.Com.Amazonaws.Dynamodb.Types.ExecuteStatementInput;
 import Dafny.Com.Amazonaws.Dynamodb.Types.ExecuteStatementOutput;
 import Dafny.Com.Amazonaws.Dynamodb.Types.ExecuteTransactionInput;
@@ -89,11 +114,16 @@ import Dafny.Com.Amazonaws.Dynamodb.Types.TransactWriteItemsInput;
 import Dafny.Com.Amazonaws.Dynamodb.Types.TransactWriteItemsOutput;
 import Dafny.Com.Amazonaws.Dynamodb.Types.UpdateItemInput;
 import Dafny.Com.Amazonaws.Dynamodb.Types.UpdateItemOutput;
+import Dafny.Com.Amazonaws.Dynamodb.Types.UpdateTableInput;
+import Dafny.Com.Amazonaws.Dynamodb.Types.UpdateTableOutput;
 import Wrappers_Compile.Option;
 import dafny.DafnyMap;
 import dafny.DafnySequence;
+import java.lang.Boolean;
 import java.lang.Character;
+import java.lang.Integer;
 import java.lang.String;
+import java.util.List;
 import java.util.Map;
 import java.util.Objects;
 import software.amazon.cryptography.dynamoDbEncryption.model.CollectionOfErrors;
@@ -127,6 +157,22 @@ public class ToDafny {
     return Error.create_CollectionOfErrors(list);
   }
 
+  public static TransactWriteItemsOutputTransformInput TransactWriteItemsOutputTransformInput(
+      software.amazon.cryptography.dynamoDbEncryption.model.TransactWriteItemsOutputTransformInput nativeValue) {
+    TransactWriteItemsOutput sdkOutput;
+    sdkOutput = Dafny.Com.Amazonaws.Dynamodb.ToDafny.TransactWriteItemsOutput(nativeValue.sdkOutput());
+    TransactWriteItemsInput originalInput;
+    originalInput = Dafny.Com.Amazonaws.Dynamodb.ToDafny.TransactWriteItemsInput(nativeValue.originalInput());
+    return new TransactWriteItemsOutputTransformInput(sdkOutput, originalInput);
+  }
+
+  public static CreateTableInputTransformInput CreateTableInputTransformInput(
+      software.amazon.cryptography.dynamoDbEncryption.model.CreateTableInputTransformInput nativeValue) {
+    CreateTableInput sdkInput;
+    sdkInput = Dafny.Com.Amazonaws.Dynamodb.ToDafny.CreateTableInput(nativeValue.sdkInput());
+    return new CreateTableInputTransformInput(sdkInput);
+  }
+
   public static DynamoDbTableEncryptionConfig DynamoDbTableEncryptionConfig(
       software.amazon.cryptography.dynamoDbEncryption.model.DynamoDbTableEncryptionConfig nativeValue) {
     DafnySequence<? extends Character> partitionKeyName;
@@ -134,6 +180,10 @@ public class ToDafny {
     Option<DafnySequence<? extends Character>> sortKeyName;
     sortKeyName = Objects.nonNull(nativeValue.sortKeyName()) ?
         Option.create_Some(software.amazon.dafny.conversion.ToDafny.Simple.CharacterSequence(nativeValue.sortKeyName()))
+        : Option.create_None();
+    Option<SearchConfig> beacons;
+    beacons = Objects.nonNull(nativeValue.beacons()) ?
+        Option.create_Some(ToDafny.SearchConfig(nativeValue.beacons()))
         : Option.create_None();
     DafnyMap<? extends DafnySequence<? extends Character>, ? extends CryptoAction> attributeActions;
     attributeActions = software.amazon.cryptography.dynamoDbItemEncryptor.ToDafny.AttributeActions(nativeValue.attributeActions());
@@ -157,7 +207,21 @@ public class ToDafny {
     cmm = Objects.nonNull(nativeValue.cmm()) ?
         Option.create_Some(software.amazon.cryptography.materialProviders.ToDafny.CryptographicMaterialsManager(nativeValue.cmm()))
         : Option.create_None();
-    return new DynamoDbTableEncryptionConfig(partitionKeyName, sortKeyName, attributeActions, allowedUnauthenticatedAttributes, allowedUnauthenticatedAttributePrefix, algorithmSuiteId, keyring, cmm);
+    return new DynamoDbTableEncryptionConfig(partitionKeyName, sortKeyName, beacons, attributeActions, allowedUnauthenticatedAttributes, allowedUnauthenticatedAttributePrefix, algorithmSuiteId, keyring, cmm);
+  }
+
+  public static CreateTableOutputTransformOutput CreateTableOutputTransformOutput(
+      software.amazon.cryptography.dynamoDbEncryption.model.CreateTableOutputTransformOutput nativeValue) {
+    CreateTableOutput transformedOutput;
+    transformedOutput = Dafny.Com.Amazonaws.Dynamodb.ToDafny.CreateTableOutput(nativeValue.transformedOutput());
+    return new CreateTableOutputTransformOutput(transformedOutput);
+  }
+
+  public static GetItemOutputTransformOutput GetItemOutputTransformOutput(
+      software.amazon.cryptography.dynamoDbEncryption.model.GetItemOutputTransformOutput nativeValue) {
+    GetItemOutput transformedOutput;
+    transformedOutput = Dafny.Com.Amazonaws.Dynamodb.ToDafny.GetItemOutput(nativeValue.transformedOutput());
+    return new GetItemOutputTransformOutput(transformedOutput);
   }
 
   public static PutItemInputTransformInput PutItemInputTransformInput(
@@ -167,13 +231,87 @@ public class ToDafny {
     return new PutItemInputTransformInput(sdkInput);
   }
 
-  public static TransactWriteItemsOutputTransformInput TransactWriteItemsOutputTransformInput(
-      software.amazon.cryptography.dynamoDbEncryption.model.TransactWriteItemsOutputTransformInput nativeValue) {
-    TransactWriteItemsOutput sdkOutput;
-    sdkOutput = Dafny.Com.Amazonaws.Dynamodb.ToDafny.TransactWriteItemsOutput(nativeValue.sdkOutput());
-    TransactWriteItemsInput originalInput;
-    originalInput = Dafny.Com.Amazonaws.Dynamodb.ToDafny.TransactWriteItemsInput(nativeValue.originalInput());
-    return new TransactWriteItemsOutputTransformInput(sdkOutput, originalInput);
+  public static NonSensitivePart NonSensitivePart(
+      software.amazon.cryptography.dynamoDbEncryption.model.NonSensitivePart nativeValue) {
+    DafnySequence<? extends Character> name;
+    name = software.amazon.dafny.conversion.ToDafny.Simple.CharacterSequence(nativeValue.name());
+    DafnySequence<? extends Character> loc;
+    loc = software.amazon.dafny.conversion.ToDafny.Simple.CharacterSequence(nativeValue.loc());
+    return new NonSensitivePart(name, loc);
+  }
+
+  public static TransactGetItemsInputTransformOutput TransactGetItemsInputTransformOutput(
+      software.amazon.cryptography.dynamoDbEncryption.model.TransactGetItemsInputTransformOutput nativeValue) {
+    TransactGetItemsInput transformedInput;
+    transformedInput = Dafny.Com.Amazonaws.Dynamodb.ToDafny.TransactGetItemsInput(nativeValue.transformedInput());
+    return new TransactGetItemsInputTransformOutput(transformedInput);
+  }
+
+  public static QueryInputTransformOutput QueryInputTransformOutput(
+      software.amazon.cryptography.dynamoDbEncryption.model.QueryInputTransformOutput nativeValue) {
+    QueryInput transformedInput;
+    transformedInput = Dafny.Com.Amazonaws.Dynamodb.ToDafny.QueryInput(nativeValue.transformedInput());
+    return new QueryInputTransformOutput(transformedInput);
+  }
+
+  public static GetItemInputTransformOutput GetItemInputTransformOutput(
+      software.amazon.cryptography.dynamoDbEncryption.model.GetItemInputTransformOutput nativeValue) {
+    GetItemInput transformedInput;
+    transformedInput = Dafny.Com.Amazonaws.Dynamodb.ToDafny.GetItemInput(nativeValue.transformedInput());
+    return new GetItemInputTransformOutput(transformedInput);
+  }
+
+  public static ExecuteTransactionInputTransformOutput ExecuteTransactionInputTransformOutput(
+      software.amazon.cryptography.dynamoDbEncryption.model.ExecuteTransactionInputTransformOutput nativeValue) {
+    ExecuteTransactionInput transformedInput;
+    transformedInput = Dafny.Com.Amazonaws.Dynamodb.ToDafny.ExecuteTransactionInput(nativeValue.transformedInput());
+    return new ExecuteTransactionInputTransformOutput(transformedInput);
+  }
+
+  public static ExecuteStatementInputTransformInput ExecuteStatementInputTransformInput(
+      software.amazon.cryptography.dynamoDbEncryption.model.ExecuteStatementInputTransformInput nativeValue) {
+    ExecuteStatementInput sdkInput;
+    sdkInput = Dafny.Com.Amazonaws.Dynamodb.ToDafny.ExecuteStatementInput(nativeValue.sdkInput());
+    return new ExecuteStatementInputTransformInput(sdkInput);
+  }
+
+  public static BatchExecuteStatementInputTransformInput BatchExecuteStatementInputTransformInput(
+      software.amazon.cryptography.dynamoDbEncryption.model.BatchExecuteStatementInputTransformInput nativeValue) {
+    BatchExecuteStatementInput sdkInput;
+    sdkInput = Dafny.Com.Amazonaws.Dynamodb.ToDafny.BatchExecuteStatementInput(nativeValue.sdkInput());
+    return new BatchExecuteStatementInputTransformInput(sdkInput);
+  }
+
+  public static TransactGetItemsOutputTransformOutput TransactGetItemsOutputTransformOutput(
+      software.amazon.cryptography.dynamoDbEncryption.model.TransactGetItemsOutputTransformOutput nativeValue) {
+    TransactGetItemsOutput transformedOutput;
+    transformedOutput = Dafny.Com.Amazonaws.Dynamodb.ToDafny.TransactGetItemsOutput(nativeValue.transformedOutput());
+    return new TransactGetItemsOutputTransformOutput(transformedOutput);
+  }
+
+  public static SearchConfig SearchConfig(
+      software.amazon.cryptography.dynamoDbEncryption.model.SearchConfig nativeValue) {
+    DafnySequence<? extends BeaconVersion> versions;
+    versions = ToDafny.BeaconVersionList(nativeValue.versions());
+    Integer writeVersion;
+    writeVersion = (nativeValue.writeVersion());
+    return new SearchConfig(versions, writeVersion);
+  }
+
+  public static VirtualField VirtualField(
+      software.amazon.cryptography.dynamoDbEncryption.model.VirtualField nativeValue) {
+    DafnySequence<? extends Character> name;
+    name = software.amazon.dafny.conversion.ToDafny.Simple.CharacterSequence(nativeValue.name());
+    DafnySequence<? extends Character> config;
+    config = software.amazon.dafny.conversion.ToDafny.Simple.CharacterSequence(nativeValue.config());
+    return new VirtualField(name, config);
+  }
+
+  public static PutItemInputTransformOutput PutItemInputTransformOutput(
+      software.amazon.cryptography.dynamoDbEncryption.model.PutItemInputTransformOutput nativeValue) {
+    PutItemInput transformedInput;
+    transformedInput = Dafny.Com.Amazonaws.Dynamodb.ToDafny.PutItemInput(nativeValue.transformedInput());
+    return new PutItemInputTransformOutput(transformedInput);
   }
 
   public static ScanOutputTransformInput ScanOutputTransformInput(
@@ -185,41 +323,55 @@ public class ToDafny {
     return new ScanOutputTransformInput(sdkOutput, originalInput);
   }
 
-  public static DeleteItemOutputTransformInput DeleteItemOutputTransformInput(
-      software.amazon.cryptography.dynamoDbEncryption.model.DeleteItemOutputTransformInput nativeValue) {
-    DeleteItemOutput sdkOutput;
-    sdkOutput = Dafny.Com.Amazonaws.Dynamodb.ToDafny.DeleteItemOutput(nativeValue.sdkOutput());
-    DeleteItemInput originalInput;
-    originalInput = Dafny.Com.Amazonaws.Dynamodb.ToDafny.DeleteItemInput(nativeValue.originalInput());
-    return new DeleteItemOutputTransformInput(sdkOutput, originalInput);
+  public static DeleteItemInputTransformInput DeleteItemInputTransformInput(
+      software.amazon.cryptography.dynamoDbEncryption.model.DeleteItemInputTransformInput nativeValue) {
+    DeleteItemInput sdkInput;
+    sdkInput = Dafny.Com.Amazonaws.Dynamodb.ToDafny.DeleteItemInput(nativeValue.sdkInput());
+    return new DeleteItemInputTransformInput(sdkInput);
   }
 
-  public static BatchExecuteStatementInputTransformInput BatchExecuteStatementInputTransformInput(
-      software.amazon.cryptography.dynamoDbEncryption.model.BatchExecuteStatementInputTransformInput nativeValue) {
-    BatchExecuteStatementInput sdkInput;
-    sdkInput = Dafny.Com.Amazonaws.Dynamodb.ToDafny.BatchExecuteStatementInput(nativeValue.sdkInput());
-    return new BatchExecuteStatementInputTransformInput(sdkInput);
+  public static QueryOutputTransformInput QueryOutputTransformInput(
+      software.amazon.cryptography.dynamoDbEncryption.model.QueryOutputTransformInput nativeValue) {
+    QueryOutput sdkOutput;
+    sdkOutput = Dafny.Com.Amazonaws.Dynamodb.ToDafny.QueryOutput(nativeValue.sdkOutput());
+    QueryInput originalInput;
+    originalInput = Dafny.Com.Amazonaws.Dynamodb.ToDafny.QueryInput(nativeValue.originalInput());
+    return new QueryOutputTransformInput(sdkOutput, originalInput);
   }
 
-  public static ExecuteStatementInputTransformOutput ExecuteStatementInputTransformOutput(
-      software.amazon.cryptography.dynamoDbEncryption.model.ExecuteStatementInputTransformOutput nativeValue) {
-    ExecuteStatementInput transformedInput;
-    transformedInput = Dafny.Com.Amazonaws.Dynamodb.ToDafny.ExecuteStatementInput(nativeValue.transformedInput());
-    return new ExecuteStatementInputTransformOutput(transformedInput);
+  public static GetItemInputTransformInput GetItemInputTransformInput(
+      software.amazon.cryptography.dynamoDbEncryption.model.GetItemInputTransformInput nativeValue) {
+    GetItemInput sdkInput;
+    sdkInput = Dafny.Com.Amazonaws.Dynamodb.ToDafny.GetItemInput(nativeValue.sdkInput());
+    return new GetItemInputTransformInput(sdkInput);
   }
 
-  public static GetItemOutputTransformOutput GetItemOutputTransformOutput(
-      software.amazon.cryptography.dynamoDbEncryption.model.GetItemOutputTransformOutput nativeValue) {
-    GetItemOutput transformedOutput;
-    transformedOutput = Dafny.Com.Amazonaws.Dynamodb.ToDafny.GetItemOutput(nativeValue.transformedOutput());
-    return new GetItemOutputTransformOutput(transformedOutput);
+  public static DescribeTableInputTransformInput DescribeTableInputTransformInput(
+      software.amazon.cryptography.dynamoDbEncryption.model.DescribeTableInputTransformInput nativeValue) {
+    DescribeTableInput sdkInput;
+    sdkInput = Dafny.Com.Amazonaws.Dynamodb.ToDafny.DescribeTableInput(nativeValue.sdkInput());
+    return new DescribeTableInputTransformInput(sdkInput);
   }
 
-  public static BatchGetItemOutputTransformOutput BatchGetItemOutputTransformOutput(
-      software.amazon.cryptography.dynamoDbEncryption.model.BatchGetItemOutputTransformOutput nativeValue) {
-    BatchGetItemOutput transformedOutput;
-    transformedOutput = Dafny.Com.Amazonaws.Dynamodb.ToDafny.BatchGetItemOutput(nativeValue.transformedOutput());
-    return new BatchGetItemOutputTransformOutput(transformedOutput);
+  public static ScanInputTransformInput ScanInputTransformInput(
+      software.amazon.cryptography.dynamoDbEncryption.model.ScanInputTransformInput nativeValue) {
+    ScanInput sdkInput;
+    sdkInput = Dafny.Com.Amazonaws.Dynamodb.ToDafny.ScanInput(nativeValue.sdkInput());
+    return new ScanInputTransformInput(sdkInput);
+  }
+
+  public static UpdateTableOutputTransformOutput UpdateTableOutputTransformOutput(
+      software.amazon.cryptography.dynamoDbEncryption.model.UpdateTableOutputTransformOutput nativeValue) {
+    UpdateTableOutput transformedOutput;
+    transformedOutput = Dafny.Com.Amazonaws.Dynamodb.ToDafny.UpdateTableOutput(nativeValue.transformedOutput());
+    return new UpdateTableOutputTransformOutput(transformedOutput);
+  }
+
+  public static DescribeTableOutputTransformOutput DescribeTableOutputTransformOutput(
+      software.amazon.cryptography.dynamoDbEncryption.model.DescribeTableOutputTransformOutput nativeValue) {
+    DescribeTableOutput transformedOutput;
+    transformedOutput = Dafny.Com.Amazonaws.Dynamodb.ToDafny.DescribeTableOutput(nativeValue.transformedOutput());
+    return new DescribeTableOutputTransformOutput(transformedOutput);
   }
 
   public static DeleteItemOutputTransformOutput DeleteItemOutputTransformOutput(
@@ -229,27 +381,50 @@ public class ToDafny {
     return new DeleteItemOutputTransformOutput(transformedOutput);
   }
 
-  public static DeleteItemInputTransformOutput DeleteItemInputTransformOutput(
-      software.amazon.cryptography.dynamoDbEncryption.model.DeleteItemInputTransformOutput nativeValue) {
-    DeleteItemInput transformedInput;
-    transformedInput = Dafny.Com.Amazonaws.Dynamodb.ToDafny.DeleteItemInput(nativeValue.transformedInput());
-    return new DeleteItemInputTransformOutput(transformedInput);
+  public static GetItemOutputTransformInput GetItemOutputTransformInput(
+      software.amazon.cryptography.dynamoDbEncryption.model.GetItemOutputTransformInput nativeValue) {
+    GetItemOutput sdkOutput;
+    sdkOutput = Dafny.Com.Amazonaws.Dynamodb.ToDafny.GetItemOutput(nativeValue.sdkOutput());
+    GetItemInput originalInput;
+    originalInput = Dafny.Com.Amazonaws.Dynamodb.ToDafny.GetItemInput(nativeValue.originalInput());
+    return new GetItemOutputTransformInput(sdkOutput, originalInput);
   }
 
-  public static UpdateItemOutputTransformOutput UpdateItemOutputTransformOutput(
-      software.amazon.cryptography.dynamoDbEncryption.model.UpdateItemOutputTransformOutput nativeValue) {
-    UpdateItemOutput transformedOutput;
-    transformedOutput = Dafny.Com.Amazonaws.Dynamodb.ToDafny.UpdateItemOutput(nativeValue.transformedOutput());
-    return new UpdateItemOutputTransformOutput(transformedOutput);
+  public static TransactWriteItemsInputTransformOutput TransactWriteItemsInputTransformOutput(
+      software.amazon.cryptography.dynamoDbEncryption.model.TransactWriteItemsInputTransformOutput nativeValue) {
+    TransactWriteItemsInput transformedInput;
+    transformedInput = Dafny.Com.Amazonaws.Dynamodb.ToDafny.TransactWriteItemsInput(nativeValue.transformedInput());
+    return new TransactWriteItemsInputTransformOutput(transformedInput);
   }
 
-  public static PutItemOutputTransformInput PutItemOutputTransformInput(
-      software.amazon.cryptography.dynamoDbEncryption.model.PutItemOutputTransformInput nativeValue) {
-    PutItemOutput sdkOutput;
-    sdkOutput = Dafny.Com.Amazonaws.Dynamodb.ToDafny.PutItemOutput(nativeValue.sdkOutput());
-    PutItemInput originalInput;
-    originalInput = Dafny.Com.Amazonaws.Dynamodb.ToDafny.PutItemInput(nativeValue.originalInput());
-    return new PutItemOutputTransformInput(sdkOutput, originalInput);
+  public static BatchGetItemOutputTransformInput BatchGetItemOutputTransformInput(
+      software.amazon.cryptography.dynamoDbEncryption.model.BatchGetItemOutputTransformInput nativeValue) {
+    BatchGetItemOutput sdkOutput;
+    sdkOutput = Dafny.Com.Amazonaws.Dynamodb.ToDafny.BatchGetItemOutput(nativeValue.sdkOutput());
+    BatchGetItemInput originalInput;
+    originalInput = Dafny.Com.Amazonaws.Dynamodb.ToDafny.BatchGetItemInput(nativeValue.originalInput());
+    return new BatchGetItemOutputTransformInput(sdkOutput, originalInput);
+  }
+
+  public static BeaconVersion BeaconVersion(
+      software.amazon.cryptography.dynamoDbEncryption.model.BeaconVersion nativeValue) {
+    Integer version;
+    version = (nativeValue.version());
+    IKeyring keyring;
+    keyring = software.amazon.cryptography.materialProviders.ToDafny.Keyring(nativeValue.keyring());
+    Option<DafnySequence<? extends StandardBeacon>> standardBeacons;
+    standardBeacons = (Objects.nonNull(nativeValue.standardBeacons()) && nativeValue.standardBeacons().size() > 0) ?
+        Option.create_Some(ToDafny.StandardBeaconList(nativeValue.standardBeacons()))
+        : Option.create_None();
+    Option<DafnySequence<? extends CompoundBeacon>> compoundBeacons;
+    compoundBeacons = (Objects.nonNull(nativeValue.compoundBeacons()) && nativeValue.compoundBeacons().size() > 0) ?
+        Option.create_Some(ToDafny.CompoundBeaconList(nativeValue.compoundBeacons()))
+        : Option.create_None();
+    Option<DafnySequence<? extends VirtualField>> virtualFields;
+    virtualFields = (Objects.nonNull(nativeValue.virtualFields()) && nativeValue.virtualFields().size() > 0) ?
+        Option.create_Some(ToDafny.VirtualFieldList(nativeValue.virtualFields()))
+        : Option.create_None();
+    return new BeaconVersion(version, keyring, standardBeacons, compoundBeacons, virtualFields);
   }
 
   public static BatchGetItemInputTransformOutput BatchGetItemInputTransformOutput(
@@ -268,94 +443,50 @@ public class ToDafny {
     return new BatchExecuteStatementOutputTransformInput(sdkOutput, originalInput);
   }
 
-  public static PutItemInputTransformOutput PutItemInputTransformOutput(
-      software.amazon.cryptography.dynamoDbEncryption.model.PutItemInputTransformOutput nativeValue) {
-    PutItemInput transformedInput;
-    transformedInput = Dafny.Com.Amazonaws.Dynamodb.ToDafny.PutItemInput(nativeValue.transformedInput());
-    return new PutItemInputTransformOutput(transformedInput);
+  public static DeleteItemOutputTransformInput DeleteItemOutputTransformInput(
+      software.amazon.cryptography.dynamoDbEncryption.model.DeleteItemOutputTransformInput nativeValue) {
+    DeleteItemOutput sdkOutput;
+    sdkOutput = Dafny.Com.Amazonaws.Dynamodb.ToDafny.DeleteItemOutput(nativeValue.sdkOutput());
+    DeleteItemInput originalInput;
+    originalInput = Dafny.Com.Amazonaws.Dynamodb.ToDafny.DeleteItemInput(nativeValue.originalInput());
+    return new DeleteItemOutputTransformInput(sdkOutput, originalInput);
   }
 
-  public static BatchGetItemOutputTransformInput BatchGetItemOutputTransformInput(
-      software.amazon.cryptography.dynamoDbEncryption.model.BatchGetItemOutputTransformInput nativeValue) {
-    BatchGetItemOutput sdkOutput;
-    sdkOutput = Dafny.Com.Amazonaws.Dynamodb.ToDafny.BatchGetItemOutput(nativeValue.sdkOutput());
-    BatchGetItemInput originalInput;
-    originalInput = Dafny.Com.Amazonaws.Dynamodb.ToDafny.BatchGetItemInput(nativeValue.originalInput());
-    return new BatchGetItemOutputTransformInput(sdkOutput, originalInput);
+  public static DynamoDbEncryptionConfig DynamoDbEncryptionConfig(
+      software.amazon.cryptography.dynamoDbEncryption.model.DynamoDbEncryptionConfig nativeValue) {
+    DafnyMap<? extends DafnySequence<? extends Character>, ? extends DynamoDbTableEncryptionConfig> tableEncryptionConfigs;
+    tableEncryptionConfigs = ToDafny.DynamoDbTableEncryptionConfigs(nativeValue.tableEncryptionConfigs());
+    return new DynamoDbEncryptionConfig(tableEncryptionConfigs);
   }
 
-  public static QueryOutputTransformInput QueryOutputTransformInput(
-      software.amazon.cryptography.dynamoDbEncryption.model.QueryOutputTransformInput nativeValue) {
-    QueryOutput sdkOutput;
-    sdkOutput = Dafny.Com.Amazonaws.Dynamodb.ToDafny.QueryOutput(nativeValue.sdkOutput());
-    QueryInput originalInput;
-    originalInput = Dafny.Com.Amazonaws.Dynamodb.ToDafny.QueryInput(nativeValue.originalInput());
-    return new QueryOutputTransformInput(sdkOutput, originalInput);
+  public static BatchExecuteStatementInputTransformOutput BatchExecuteStatementInputTransformOutput(
+      software.amazon.cryptography.dynamoDbEncryption.model.BatchExecuteStatementInputTransformOutput nativeValue) {
+    BatchExecuteStatementInput transformedInput;
+    transformedInput = Dafny.Com.Amazonaws.Dynamodb.ToDafny.BatchExecuteStatementInput(nativeValue.transformedInput());
+    return new BatchExecuteStatementInputTransformOutput(transformedInput);
   }
 
-  public static DeleteItemInputTransformInput DeleteItemInputTransformInput(
-      software.amazon.cryptography.dynamoDbEncryption.model.DeleteItemInputTransformInput nativeValue) {
-    DeleteItemInput sdkInput;
-    sdkInput = Dafny.Com.Amazonaws.Dynamodb.ToDafny.DeleteItemInput(nativeValue.sdkInput());
-    return new DeleteItemInputTransformInput(sdkInput);
+  public static UpdateItemOutputTransformOutput UpdateItemOutputTransformOutput(
+      software.amazon.cryptography.dynamoDbEncryption.model.UpdateItemOutputTransformOutput nativeValue) {
+    UpdateItemOutput transformedOutput;
+    transformedOutput = Dafny.Com.Amazonaws.Dynamodb.ToDafny.UpdateItemOutput(nativeValue.transformedOutput());
+    return new UpdateItemOutputTransformOutput(transformedOutput);
   }
 
-  public static TransactWriteItemsInputTransformOutput TransactWriteItemsInputTransformOutput(
-      software.amazon.cryptography.dynamoDbEncryption.model.TransactWriteItemsInputTransformOutput nativeValue) {
-    TransactWriteItemsInput transformedInput;
-    transformedInput = Dafny.Com.Amazonaws.Dynamodb.ToDafny.TransactWriteItemsInput(nativeValue.transformedInput());
-    return new TransactWriteItemsInputTransformOutput(transformedInput);
+  public static DeleteItemInputTransformOutput DeleteItemInputTransformOutput(
+      software.amazon.cryptography.dynamoDbEncryption.model.DeleteItemInputTransformOutput nativeValue) {
+    DeleteItemInput transformedInput;
+    transformedInput = Dafny.Com.Amazonaws.Dynamodb.ToDafny.DeleteItemInput(nativeValue.transformedInput());
+    return new DeleteItemInputTransformOutput(transformedInput);
   }
 
-  public static GetItemInputTransformOutput GetItemInputTransformOutput(
-      software.amazon.cryptography.dynamoDbEncryption.model.GetItemInputTransformOutput nativeValue) {
-    GetItemInput transformedInput;
-    transformedInput = Dafny.Com.Amazonaws.Dynamodb.ToDafny.GetItemInput(nativeValue.transformedInput());
-    return new GetItemInputTransformOutput(transformedInput);
-  }
-
-  public static GetItemInputTransformInput GetItemInputTransformInput(
-      software.amazon.cryptography.dynamoDbEncryption.model.GetItemInputTransformInput nativeValue) {
-    GetItemInput sdkInput;
-    sdkInput = Dafny.Com.Amazonaws.Dynamodb.ToDafny.GetItemInput(nativeValue.sdkInput());
-    return new GetItemInputTransformInput(sdkInput);
-  }
-
-  public static QueryInputTransformOutput QueryInputTransformOutput(
-      software.amazon.cryptography.dynamoDbEncryption.model.QueryInputTransformOutput nativeValue) {
-    QueryInput transformedInput;
-    transformedInput = Dafny.Com.Amazonaws.Dynamodb.ToDafny.QueryInput(nativeValue.transformedInput());
-    return new QueryInputTransformOutput(transformedInput);
-  }
-
-  public static BatchWriteItemOutputTransformOutput BatchWriteItemOutputTransformOutput(
-      software.amazon.cryptography.dynamoDbEncryption.model.BatchWriteItemOutputTransformOutput nativeValue) {
-    BatchWriteItemOutput transformedOutput;
-    transformedOutput = Dafny.Com.Amazonaws.Dynamodb.ToDafny.BatchWriteItemOutput(nativeValue.transformedOutput());
-    return new BatchWriteItemOutputTransformOutput(transformedOutput);
-  }
-
-  public static GetItemOutputTransformInput GetItemOutputTransformInput(
-      software.amazon.cryptography.dynamoDbEncryption.model.GetItemOutputTransformInput nativeValue) {
-    GetItemOutput sdkOutput;
-    sdkOutput = Dafny.Com.Amazonaws.Dynamodb.ToDafny.GetItemOutput(nativeValue.sdkOutput());
-    GetItemInput originalInput;
-    originalInput = Dafny.Com.Amazonaws.Dynamodb.ToDafny.GetItemInput(nativeValue.originalInput());
-    return new GetItemOutputTransformInput(sdkOutput, originalInput);
-  }
-
-  public static PutItemOutputTransformOutput PutItemOutputTransformOutput(
-      software.amazon.cryptography.dynamoDbEncryption.model.PutItemOutputTransformOutput nativeValue) {
-    PutItemOutput transformedOutput;
-    transformedOutput = Dafny.Com.Amazonaws.Dynamodb.ToDafny.PutItemOutput(nativeValue.transformedOutput());
-    return new PutItemOutputTransformOutput(transformedOutput);
-  }
-
-  public static ExecuteTransactionOutputTransformOutput ExecuteTransactionOutputTransformOutput(
-      software.amazon.cryptography.dynamoDbEncryption.model.ExecuteTransactionOutputTransformOutput nativeValue) {
-    ExecuteTransactionOutput transformedOutput;
-    transformedOutput = Dafny.Com.Amazonaws.Dynamodb.ToDafny.ExecuteTransactionOutput(nativeValue.transformedOutput());
-    return new ExecuteTransactionOutputTransformOutput(transformedOutput);
+  public static UpdateTableOutputTransformInput UpdateTableOutputTransformInput(
+      software.amazon.cryptography.dynamoDbEncryption.model.UpdateTableOutputTransformInput nativeValue) {
+    UpdateTableOutput sdkOutput;
+    sdkOutput = Dafny.Com.Amazonaws.Dynamodb.ToDafny.UpdateTableOutput(nativeValue.sdkOutput());
+    UpdateTableInput originalInput;
+    originalInput = Dafny.Com.Amazonaws.Dynamodb.ToDafny.UpdateTableInput(nativeValue.originalInput());
+    return new UpdateTableOutputTransformInput(sdkOutput, originalInput);
   }
 
   public static ExecuteStatementOutputTransformOutput ExecuteStatementOutputTransformOutput(
@@ -365,6 +496,79 @@ public class ToDafny {
     return new ExecuteStatementOutputTransformOutput(transformedOutput);
   }
 
+  public static UpdateItemInputTransformOutput UpdateItemInputTransformOutput(
+      software.amazon.cryptography.dynamoDbEncryption.model.UpdateItemInputTransformOutput nativeValue) {
+    UpdateItemInput transformedInput;
+    transformedInput = Dafny.Com.Amazonaws.Dynamodb.ToDafny.UpdateItemInput(nativeValue.transformedInput());
+    return new UpdateItemInputTransformOutput(transformedInput);
+  }
+
+  public static StandardBeacon StandardBeacon(
+      software.amazon.cryptography.dynamoDbEncryption.model.StandardBeacon nativeValue) {
+    DafnySequence<? extends Character> name;
+    name = software.amazon.dafny.conversion.ToDafny.Simple.CharacterSequence(nativeValue.name());
+    Integer length;
+    length = (nativeValue.length());
+    DafnySequence<? extends Character> loc;
+    loc = software.amazon.dafny.conversion.ToDafny.Simple.CharacterSequence(nativeValue.loc());
+    return new StandardBeacon(name, length, loc);
+  }
+
+  public static ExecuteTransactionOutputTransformOutput ExecuteTransactionOutputTransformOutput(
+      software.amazon.cryptography.dynamoDbEncryption.model.ExecuteTransactionOutputTransformOutput nativeValue) {
+    ExecuteTransactionOutput transformedOutput;
+    transformedOutput = Dafny.Com.Amazonaws.Dynamodb.ToDafny.ExecuteTransactionOutput(nativeValue.transformedOutput());
+    return new ExecuteTransactionOutputTransformOutput(transformedOutput);
+  }
+
+  public static SensitivePart SensitivePart(
+      software.amazon.cryptography.dynamoDbEncryption.model.SensitivePart nativeValue) {
+    DafnySequence<? extends Character> name;
+    name = software.amazon.dafny.conversion.ToDafny.Simple.CharacterSequence(nativeValue.name());
+    Integer length;
+    length = (nativeValue.length());
+    DafnySequence<? extends Character> loc;
+    loc = software.amazon.dafny.conversion.ToDafny.Simple.CharacterSequence(nativeValue.loc());
+    return new SensitivePart(name, length, loc);
+  }
+
+  public static Constructor Constructor(
+      software.amazon.cryptography.dynamoDbEncryption.model.Constructor nativeValue) {
+    DafnySequence<? extends ConstructorPart> parts;
+    parts = ToDafny.ConstructorPartList(nativeValue.parts());
+    return new Constructor(parts);
+  }
+
+  public static ConstructorPart ConstructorPart(
+      software.amazon.cryptography.dynamoDbEncryption.model.ConstructorPart nativeValue) {
+    DafnySequence<? extends Character> name;
+    name = software.amazon.dafny.conversion.ToDafny.Simple.CharacterSequence(nativeValue.name());
+    Boolean required;
+    required = (nativeValue.required());
+    return new ConstructorPart(name, required);
+  }
+
+  public static UpdateTableInputTransformInput UpdateTableInputTransformInput(
+      software.amazon.cryptography.dynamoDbEncryption.model.UpdateTableInputTransformInput nativeValue) {
+    UpdateTableInput sdkInput;
+    sdkInput = Dafny.Com.Amazonaws.Dynamodb.ToDafny.UpdateTableInput(nativeValue.sdkInput());
+    return new UpdateTableInputTransformInput(sdkInput);
+  }
+
+  public static TransactGetItemsInputTransformInput TransactGetItemsInputTransformInput(
+      software.amazon.cryptography.dynamoDbEncryption.model.TransactGetItemsInputTransformInput nativeValue) {
+    TransactGetItemsInput sdkInput;
+    sdkInput = Dafny.Com.Amazonaws.Dynamodb.ToDafny.TransactGetItemsInput(nativeValue.sdkInput());
+    return new TransactGetItemsInputTransformInput(sdkInput);
+  }
+
+  public static PutItemOutputTransformOutput PutItemOutputTransformOutput(
+      software.amazon.cryptography.dynamoDbEncryption.model.PutItemOutputTransformOutput nativeValue) {
+    PutItemOutput transformedOutput;
+    transformedOutput = Dafny.Com.Amazonaws.Dynamodb.ToDafny.PutItemOutput(nativeValue.transformedOutput());
+    return new PutItemOutputTransformOutput(transformedOutput);
+  }
+
   public static QueryOutputTransformOutput QueryOutputTransformOutput(
       software.amazon.cryptography.dynamoDbEncryption.model.QueryOutputTransformOutput nativeValue) {
     QueryOutput transformedOutput;
@@ -372,11 +576,44 @@ public class ToDafny {
     return new QueryOutputTransformOutput(transformedOutput);
   }
 
-  public static BatchExecuteStatementInputTransformOutput BatchExecuteStatementInputTransformOutput(
-      software.amazon.cryptography.dynamoDbEncryption.model.BatchExecuteStatementInputTransformOutput nativeValue) {
-    BatchExecuteStatementInput transformedInput;
-    transformedInput = Dafny.Com.Amazonaws.Dynamodb.ToDafny.BatchExecuteStatementInput(nativeValue.transformedInput());
-    return new BatchExecuteStatementInputTransformOutput(transformedInput);
+  public static UpdateItemInputTransformInput UpdateItemInputTransformInput(
+      software.amazon.cryptography.dynamoDbEncryption.model.UpdateItemInputTransformInput nativeValue) {
+    UpdateItemInput sdkInput;
+    sdkInput = Dafny.Com.Amazonaws.Dynamodb.ToDafny.UpdateItemInput(nativeValue.sdkInput());
+    return new UpdateItemInputTransformInput(sdkInput);
+  }
+
+  public static CompoundBeacon CompoundBeacon(
+      software.amazon.cryptography.dynamoDbEncryption.model.CompoundBeacon nativeValue) {
+    DafnySequence<? extends Character> name;
+    name = software.amazon.dafny.conversion.ToDafny.Simple.CharacterSequence(nativeValue.name());
+    DafnySequence<? extends Character> split;
+    split = software.amazon.dafny.conversion.ToDafny.Simple.CharacterSequence(nativeValue.split());
+    DafnySequence<? extends SensitivePart> sensitive;
+    sensitive = ToDafny.SensitivePartsList(nativeValue.sensitive());
+    Option<DafnySequence<? extends NonSensitivePart>> nonSensitive;
+    nonSensitive = (Objects.nonNull(nativeValue.nonSensitive()) && nativeValue.nonSensitive().size() > 0) ?
+        Option.create_Some(ToDafny.NonSensitivePartsList(nativeValue.nonSensitive()))
+        : Option.create_None();
+    Option<DafnySequence<? extends Constructor>> constructors;
+    constructors = (Objects.nonNull(nativeValue.constructors()) && nativeValue.constructors().size() > 0) ?
+        Option.create_Some(ToDafny.ConstructorList(nativeValue.constructors()))
+        : Option.create_None();
+    return new CompoundBeacon(name, split, sensitive, nonSensitive, constructors);
+  }
+
+  public static BatchWriteItemOutputTransformOutput BatchWriteItemOutputTransformOutput(
+      software.amazon.cryptography.dynamoDbEncryption.model.BatchWriteItemOutputTransformOutput nativeValue) {
+    BatchWriteItemOutput transformedOutput;
+    transformedOutput = Dafny.Com.Amazonaws.Dynamodb.ToDafny.BatchWriteItemOutput(nativeValue.transformedOutput());
+    return new BatchWriteItemOutputTransformOutput(transformedOutput);
+  }
+
+  public static ScanOutputTransformOutput ScanOutputTransformOutput(
+      software.amazon.cryptography.dynamoDbEncryption.model.ScanOutputTransformOutput nativeValue) {
+    ScanOutput transformedOutput;
+    transformedOutput = Dafny.Com.Amazonaws.Dynamodb.ToDafny.ScanOutput(nativeValue.transformedOutput());
+    return new ScanOutputTransformOutput(transformedOutput);
   }
 
   public static TransactWriteItemsInputTransformInput TransactWriteItemsInputTransformInput(
@@ -393,27 +630,123 @@ public class ToDafny {
     return new BatchGetItemInputTransformInput(sdkInput);
   }
 
-  public static ExecuteStatementOutputTransformInput ExecuteStatementOutputTransformInput(
-      software.amazon.cryptography.dynamoDbEncryption.model.ExecuteStatementOutputTransformInput nativeValue) {
-    ExecuteStatementOutput sdkOutput;
-    sdkOutput = Dafny.Com.Amazonaws.Dynamodb.ToDafny.ExecuteStatementOutput(nativeValue.sdkOutput());
-    ExecuteStatementInput originalInput;
-    originalInput = Dafny.Com.Amazonaws.Dynamodb.ToDafny.ExecuteStatementInput(nativeValue.originalInput());
-    return new ExecuteStatementOutputTransformInput(sdkOutput, originalInput);
+  public static UpdateItemOutputTransformInput UpdateItemOutputTransformInput(
+      software.amazon.cryptography.dynamoDbEncryption.model.UpdateItemOutputTransformInput nativeValue) {
+    UpdateItemOutput sdkOutput;
+    sdkOutput = Dafny.Com.Amazonaws.Dynamodb.ToDafny.UpdateItemOutput(nativeValue.sdkOutput());
+    UpdateItemInput originalInput;
+    originalInput = Dafny.Com.Amazonaws.Dynamodb.ToDafny.UpdateItemInput(nativeValue.originalInput());
+    return new UpdateItemOutputTransformInput(sdkOutput, originalInput);
   }
 
-  public static ScanOutputTransformOutput ScanOutputTransformOutput(
-      software.amazon.cryptography.dynamoDbEncryption.model.ScanOutputTransformOutput nativeValue) {
-    ScanOutput transformedOutput;
-    transformedOutput = Dafny.Com.Amazonaws.Dynamodb.ToDafny.ScanOutput(nativeValue.transformedOutput());
-    return new ScanOutputTransformOutput(transformedOutput);
+  public static UpdateTableInputTransformOutput UpdateTableInputTransformOutput(
+      software.amazon.cryptography.dynamoDbEncryption.model.UpdateTableInputTransformOutput nativeValue) {
+    UpdateTableInput transformedInput;
+    transformedInput = Dafny.Com.Amazonaws.Dynamodb.ToDafny.UpdateTableInput(nativeValue.transformedInput());
+    return new UpdateTableInputTransformOutput(transformedInput);
   }
 
-  public static UpdateItemInputTransformInput UpdateItemInputTransformInput(
-      software.amazon.cryptography.dynamoDbEncryption.model.UpdateItemInputTransformInput nativeValue) {
-    UpdateItemInput sdkInput;
-    sdkInput = Dafny.Com.Amazonaws.Dynamodb.ToDafny.UpdateItemInput(nativeValue.sdkInput());
-    return new UpdateItemInputTransformInput(sdkInput);
+  public static QueryInputTransformInput QueryInputTransformInput(
+      software.amazon.cryptography.dynamoDbEncryption.model.QueryInputTransformInput nativeValue) {
+    QueryInput sdkInput;
+    sdkInput = Dafny.Com.Amazonaws.Dynamodb.ToDafny.QueryInput(nativeValue.sdkInput());
+    return new QueryInputTransformInput(sdkInput);
+  }
+
+  public static PutItemOutputTransformInput PutItemOutputTransformInput(
+      software.amazon.cryptography.dynamoDbEncryption.model.PutItemOutputTransformInput nativeValue) {
+    PutItemOutput sdkOutput;
+    sdkOutput = Dafny.Com.Amazonaws.Dynamodb.ToDafny.PutItemOutput(nativeValue.sdkOutput());
+    PutItemInput originalInput;
+    originalInput = Dafny.Com.Amazonaws.Dynamodb.ToDafny.PutItemInput(nativeValue.originalInput());
+    return new PutItemOutputTransformInput(sdkOutput, originalInput);
+  }
+
+  public static TransactGetItemsOutputTransformInput TransactGetItemsOutputTransformInput(
+      software.amazon.cryptography.dynamoDbEncryption.model.TransactGetItemsOutputTransformInput nativeValue) {
+    TransactGetItemsOutput sdkOutput;
+    sdkOutput = Dafny.Com.Amazonaws.Dynamodb.ToDafny.TransactGetItemsOutput(nativeValue.sdkOutput());
+    TransactGetItemsInput originalInput;
+    originalInput = Dafny.Com.Amazonaws.Dynamodb.ToDafny.TransactGetItemsInput(nativeValue.originalInput());
+    return new TransactGetItemsOutputTransformInput(sdkOutput, originalInput);
+  }
+
+  public static BatchWriteItemOutputTransformInput BatchWriteItemOutputTransformInput(
+      software.amazon.cryptography.dynamoDbEncryption.model.BatchWriteItemOutputTransformInput nativeValue) {
+    BatchWriteItemOutput sdkOutput;
+    sdkOutput = Dafny.Com.Amazonaws.Dynamodb.ToDafny.BatchWriteItemOutput(nativeValue.sdkOutput());
+    BatchWriteItemInput originalInput;
+    originalInput = Dafny.Com.Amazonaws.Dynamodb.ToDafny.BatchWriteItemInput(nativeValue.originalInput());
+    return new BatchWriteItemOutputTransformInput(sdkOutput, originalInput);
+  }
+
+  public static ScanInputTransformOutput ScanInputTransformOutput(
+      software.amazon.cryptography.dynamoDbEncryption.model.ScanInputTransformOutput nativeValue) {
+    ScanInput transformedInput;
+    transformedInput = Dafny.Com.Amazonaws.Dynamodb.ToDafny.ScanInput(nativeValue.transformedInput());
+    return new ScanInputTransformOutput(transformedInput);
+  }
+
+  public static CreateTableOutputTransformInput CreateTableOutputTransformInput(
+      software.amazon.cryptography.dynamoDbEncryption.model.CreateTableOutputTransformInput nativeValue) {
+    CreateTableOutput sdkOutput;
+    sdkOutput = Dafny.Com.Amazonaws.Dynamodb.ToDafny.CreateTableOutput(nativeValue.sdkOutput());
+    CreateTableInput originalInput;
+    originalInput = Dafny.Com.Amazonaws.Dynamodb.ToDafny.CreateTableInput(nativeValue.originalInput());
+    return new CreateTableOutputTransformInput(sdkOutput, originalInput);
+  }
+
+  public static ExecuteTransactionOutputTransformInput ExecuteTransactionOutputTransformInput(
+      software.amazon.cryptography.dynamoDbEncryption.model.ExecuteTransactionOutputTransformInput nativeValue) {
+    ExecuteTransactionOutput sdkOutput;
+    sdkOutput = Dafny.Com.Amazonaws.Dynamodb.ToDafny.ExecuteTransactionOutput(nativeValue.sdkOutput());
+    ExecuteTransactionInput originalInput;
+    originalInput = Dafny.Com.Amazonaws.Dynamodb.ToDafny.ExecuteTransactionInput(nativeValue.originalInput());
+    return new ExecuteTransactionOutputTransformInput(sdkOutput, originalInput);
+  }
+
+  public static DescribeTableOutputTransformInput DescribeTableOutputTransformInput(
+      software.amazon.cryptography.dynamoDbEncryption.model.DescribeTableOutputTransformInput nativeValue) {
+    DescribeTableOutput sdkOutput;
+    sdkOutput = Dafny.Com.Amazonaws.Dynamodb.ToDafny.DescribeTableOutput(nativeValue.sdkOutput());
+    DescribeTableInput originalInput;
+    originalInput = Dafny.Com.Amazonaws.Dynamodb.ToDafny.DescribeTableInput(nativeValue.originalInput());
+    return new DescribeTableOutputTransformInput(sdkOutput, originalInput);
+  }
+
+  public static BatchWriteItemInputTransformInput BatchWriteItemInputTransformInput(
+      software.amazon.cryptography.dynamoDbEncryption.model.BatchWriteItemInputTransformInput nativeValue) {
+    BatchWriteItemInput sdkInput;
+    sdkInput = Dafny.Com.Amazonaws.Dynamodb.ToDafny.BatchWriteItemInput(nativeValue.sdkInput());
+    return new BatchWriteItemInputTransformInput(sdkInput);
+  }
+
+  public static DescribeTableInputTransformOutput DescribeTableInputTransformOutput(
+      software.amazon.cryptography.dynamoDbEncryption.model.DescribeTableInputTransformOutput nativeValue) {
+    DescribeTableInput transformedInput;
+    transformedInput = Dafny.Com.Amazonaws.Dynamodb.ToDafny.DescribeTableInput(nativeValue.transformedInput());
+    return new DescribeTableInputTransformOutput(transformedInput);
+  }
+
+  public static ExecuteStatementInputTransformOutput ExecuteStatementInputTransformOutput(
+      software.amazon.cryptography.dynamoDbEncryption.model.ExecuteStatementInputTransformOutput nativeValue) {
+    ExecuteStatementInput transformedInput;
+    transformedInput = Dafny.Com.Amazonaws.Dynamodb.ToDafny.ExecuteStatementInput(nativeValue.transformedInput());
+    return new ExecuteStatementInputTransformOutput(transformedInput);
+  }
+
+  public static BatchGetItemOutputTransformOutput BatchGetItemOutputTransformOutput(
+      software.amazon.cryptography.dynamoDbEncryption.model.BatchGetItemOutputTransformOutput nativeValue) {
+    BatchGetItemOutput transformedOutput;
+    transformedOutput = Dafny.Com.Amazonaws.Dynamodb.ToDafny.BatchGetItemOutput(nativeValue.transformedOutput());
+    return new BatchGetItemOutputTransformOutput(transformedOutput);
+  }
+
+  public static CreateTableInputTransformOutput CreateTableInputTransformOutput(
+      software.amazon.cryptography.dynamoDbEncryption.model.CreateTableInputTransformOutput nativeValue) {
+    CreateTableInput transformedInput;
+    transformedInput = Dafny.Com.Amazonaws.Dynamodb.ToDafny.CreateTableInput(nativeValue.transformedInput());
+    return new CreateTableInputTransformOutput(transformedInput);
   }
 
   public static BatchWriteItemInputTransformOutput BatchWriteItemInputTransformOutput(
@@ -421,27 +754,6 @@ public class ToDafny {
     BatchWriteItemInput transformedInput;
     transformedInput = Dafny.Com.Amazonaws.Dynamodb.ToDafny.BatchWriteItemInput(nativeValue.transformedInput());
     return new BatchWriteItemInputTransformOutput(transformedInput);
-  }
-
-  public static TransactWriteItemsOutputTransformOutput TransactWriteItemsOutputTransformOutput(
-      software.amazon.cryptography.dynamoDbEncryption.model.TransactWriteItemsOutputTransformOutput nativeValue) {
-    TransactWriteItemsOutput transformedOutput;
-    transformedOutput = Dafny.Com.Amazonaws.Dynamodb.ToDafny.TransactWriteItemsOutput(nativeValue.transformedOutput());
-    return new TransactWriteItemsOutputTransformOutput(transformedOutput);
-  }
-
-  public static TransactGetItemsInputTransformInput TransactGetItemsInputTransformInput(
-      software.amazon.cryptography.dynamoDbEncryption.model.TransactGetItemsInputTransformInput nativeValue) {
-    TransactGetItemsInput sdkInput;
-    sdkInput = Dafny.Com.Amazonaws.Dynamodb.ToDafny.TransactGetItemsInput(nativeValue.sdkInput());
-    return new TransactGetItemsInputTransformInput(sdkInput);
-  }
-
-  public static DynamoDbEncryptionConfig DynamoDbEncryptionConfig(
-      software.amazon.cryptography.dynamoDbEncryption.model.DynamoDbEncryptionConfig nativeValue) {
-    DafnyMap<? extends DafnySequence<? extends Character>, ? extends DynamoDbTableEncryptionConfig> tableEncryptionConfigs;
-    tableEncryptionConfigs = ToDafny.DynamoDbTableEncryptionConfigs(nativeValue.tableEncryptionConfigs());
-    return new DynamoDbEncryptionConfig(tableEncryptionConfigs);
   }
 
   public static BatchExecuteStatementOutputTransformOutput BatchExecuteStatementOutputTransformOutput(
@@ -458,109 +770,90 @@ public class ToDafny {
     return new ExecuteTransactionInputTransformInput(sdkInput);
   }
 
-  public static TransactGetItemsOutputTransformInput TransactGetItemsOutputTransformInput(
-      software.amazon.cryptography.dynamoDbEncryption.model.TransactGetItemsOutputTransformInput nativeValue) {
-    TransactGetItemsOutput sdkOutput;
-    sdkOutput = Dafny.Com.Amazonaws.Dynamodb.ToDafny.TransactGetItemsOutput(nativeValue.sdkOutput());
-    TransactGetItemsInput originalInput;
-    originalInput = Dafny.Com.Amazonaws.Dynamodb.ToDafny.TransactGetItemsInput(nativeValue.originalInput());
-    return new TransactGetItemsOutputTransformInput(sdkOutput, originalInput);
+  public static ExecuteStatementOutputTransformInput ExecuteStatementOutputTransformInput(
+      software.amazon.cryptography.dynamoDbEncryption.model.ExecuteStatementOutputTransformInput nativeValue) {
+    ExecuteStatementOutput sdkOutput;
+    sdkOutput = Dafny.Com.Amazonaws.Dynamodb.ToDafny.ExecuteStatementOutput(nativeValue.sdkOutput());
+    ExecuteStatementInput originalInput;
+    originalInput = Dafny.Com.Amazonaws.Dynamodb.ToDafny.ExecuteStatementInput(nativeValue.originalInput());
+    return new ExecuteStatementOutputTransformInput(sdkOutput, originalInput);
   }
 
-  public static UpdateItemOutputTransformInput UpdateItemOutputTransformInput(
-      software.amazon.cryptography.dynamoDbEncryption.model.UpdateItemOutputTransformInput nativeValue) {
-    UpdateItemOutput sdkOutput;
-    sdkOutput = Dafny.Com.Amazonaws.Dynamodb.ToDafny.UpdateItemOutput(nativeValue.sdkOutput());
-    UpdateItemInput originalInput;
-    originalInput = Dafny.Com.Amazonaws.Dynamodb.ToDafny.UpdateItemInput(nativeValue.originalInput());
-    return new UpdateItemOutputTransformInput(sdkOutput, originalInput);
-  }
-
-  public static BatchWriteItemInputTransformInput BatchWriteItemInputTransformInput(
-      software.amazon.cryptography.dynamoDbEncryption.model.BatchWriteItemInputTransformInput nativeValue) {
-    BatchWriteItemInput sdkInput;
-    sdkInput = Dafny.Com.Amazonaws.Dynamodb.ToDafny.BatchWriteItemInput(nativeValue.sdkInput());
-    return new BatchWriteItemInputTransformInput(sdkInput);
-  }
-
-  public static ScanInputTransformInput ScanInputTransformInput(
-      software.amazon.cryptography.dynamoDbEncryption.model.ScanInputTransformInput nativeValue) {
-    ScanInput sdkInput;
-    sdkInput = Dafny.Com.Amazonaws.Dynamodb.ToDafny.ScanInput(nativeValue.sdkInput());
-    return new ScanInputTransformInput(sdkInput);
-  }
-
-  public static BatchWriteItemOutputTransformInput BatchWriteItemOutputTransformInput(
-      software.amazon.cryptography.dynamoDbEncryption.model.BatchWriteItemOutputTransformInput nativeValue) {
-    BatchWriteItemOutput sdkOutput;
-    sdkOutput = Dafny.Com.Amazonaws.Dynamodb.ToDafny.BatchWriteItemOutput(nativeValue.sdkOutput());
-    BatchWriteItemInput originalInput;
-    originalInput = Dafny.Com.Amazonaws.Dynamodb.ToDafny.BatchWriteItemInput(nativeValue.originalInput());
-    return new BatchWriteItemOutputTransformInput(sdkOutput, originalInput);
-  }
-
-  public static QueryInputTransformInput QueryInputTransformInput(
-      software.amazon.cryptography.dynamoDbEncryption.model.QueryInputTransformInput nativeValue) {
-    QueryInput sdkInput;
-    sdkInput = Dafny.Com.Amazonaws.Dynamodb.ToDafny.QueryInput(nativeValue.sdkInput());
-    return new QueryInputTransformInput(sdkInput);
-  }
-
-  public static TransactGetItemsInputTransformOutput TransactGetItemsInputTransformOutput(
-      software.amazon.cryptography.dynamoDbEncryption.model.TransactGetItemsInputTransformOutput nativeValue) {
-    TransactGetItemsInput transformedInput;
-    transformedInput = Dafny.Com.Amazonaws.Dynamodb.ToDafny.TransactGetItemsInput(nativeValue.transformedInput());
-    return new TransactGetItemsInputTransformOutput(transformedInput);
-  }
-
-  public static TransactGetItemsOutputTransformOutput TransactGetItemsOutputTransformOutput(
-      software.amazon.cryptography.dynamoDbEncryption.model.TransactGetItemsOutputTransformOutput nativeValue) {
-    TransactGetItemsOutput transformedOutput;
-    transformedOutput = Dafny.Com.Amazonaws.Dynamodb.ToDafny.TransactGetItemsOutput(nativeValue.transformedOutput());
-    return new TransactGetItemsOutputTransformOutput(transformedOutput);
-  }
-
-  public static ExecuteStatementInputTransformInput ExecuteStatementInputTransformInput(
-      software.amazon.cryptography.dynamoDbEncryption.model.ExecuteStatementInputTransformInput nativeValue) {
-    ExecuteStatementInput sdkInput;
-    sdkInput = Dafny.Com.Amazonaws.Dynamodb.ToDafny.ExecuteStatementInput(nativeValue.sdkInput());
-    return new ExecuteStatementInputTransformInput(sdkInput);
-  }
-
-  public static ExecuteTransactionInputTransformOutput ExecuteTransactionInputTransformOutput(
-      software.amazon.cryptography.dynamoDbEncryption.model.ExecuteTransactionInputTransformOutput nativeValue) {
-    ExecuteTransactionInput transformedInput;
-    transformedInput = Dafny.Com.Amazonaws.Dynamodb.ToDafny.ExecuteTransactionInput(nativeValue.transformedInput());
-    return new ExecuteTransactionInputTransformOutput(transformedInput);
-  }
-
-  public static UpdateItemInputTransformOutput UpdateItemInputTransformOutput(
-      software.amazon.cryptography.dynamoDbEncryption.model.UpdateItemInputTransformOutput nativeValue) {
-    UpdateItemInput transformedInput;
-    transformedInput = Dafny.Com.Amazonaws.Dynamodb.ToDafny.UpdateItemInput(nativeValue.transformedInput());
-    return new UpdateItemInputTransformOutput(transformedInput);
-  }
-
-  public static ExecuteTransactionOutputTransformInput ExecuteTransactionOutputTransformInput(
-      software.amazon.cryptography.dynamoDbEncryption.model.ExecuteTransactionOutputTransformInput nativeValue) {
-    ExecuteTransactionOutput sdkOutput;
-    sdkOutput = Dafny.Com.Amazonaws.Dynamodb.ToDafny.ExecuteTransactionOutput(nativeValue.sdkOutput());
-    ExecuteTransactionInput originalInput;
-    originalInput = Dafny.Com.Amazonaws.Dynamodb.ToDafny.ExecuteTransactionInput(nativeValue.originalInput());
-    return new ExecuteTransactionOutputTransformInput(sdkOutput, originalInput);
-  }
-
-  public static ScanInputTransformOutput ScanInputTransformOutput(
-      software.amazon.cryptography.dynamoDbEncryption.model.ScanInputTransformOutput nativeValue) {
-    ScanInput transformedInput;
-    transformedInput = Dafny.Com.Amazonaws.Dynamodb.ToDafny.ScanInput(nativeValue.transformedInput());
-    return new ScanInputTransformOutput(transformedInput);
+  public static TransactWriteItemsOutputTransformOutput TransactWriteItemsOutputTransformOutput(
+      software.amazon.cryptography.dynamoDbEncryption.model.TransactWriteItemsOutputTransformOutput nativeValue) {
+    TransactWriteItemsOutput transformedOutput;
+    transformedOutput = Dafny.Com.Amazonaws.Dynamodb.ToDafny.TransactWriteItemsOutput(nativeValue.transformedOutput());
+    return new TransactWriteItemsOutputTransformOutput(transformedOutput);
   }
 
   public static Error Error(DynamoDbEncryptionException nativeValue) {
     DafnySequence<? extends Character> message;
     message = software.amazon.dafny.conversion.ToDafny.Simple.CharacterSequence(nativeValue.message());
     return new Error_DynamoDbEncryptionException(message);
+  }
+
+  public static DafnySequence<? extends VirtualField> VirtualFieldList(
+      List<software.amazon.cryptography.dynamoDbEncryption.model.VirtualField> nativeValue) {
+    return software.amazon.dafny.conversion.ToDafny.Aggregate.GenericToSequence(
+        nativeValue, 
+        software.amazon.cryptography.dynamoDbEncryption.ToDafny::VirtualField, 
+        VirtualField._typeDescriptor());
+  }
+
+  public static DafnySequence<? extends StandardBeacon> StandardBeaconList(
+      List<software.amazon.cryptography.dynamoDbEncryption.model.StandardBeacon> nativeValue) {
+    return software.amazon.dafny.conversion.ToDafny.Aggregate.GenericToSequence(
+        nativeValue, 
+        software.amazon.cryptography.dynamoDbEncryption.ToDafny::StandardBeacon, 
+        StandardBeacon._typeDescriptor());
+  }
+
+  public static DafnySequence<? extends NonSensitivePart> NonSensitivePartsList(
+      List<software.amazon.cryptography.dynamoDbEncryption.model.NonSensitivePart> nativeValue) {
+    return software.amazon.dafny.conversion.ToDafny.Aggregate.GenericToSequence(
+        nativeValue, 
+        software.amazon.cryptography.dynamoDbEncryption.ToDafny::NonSensitivePart, 
+        NonSensitivePart._typeDescriptor());
+  }
+
+  public static DafnySequence<? extends SensitivePart> SensitivePartsList(
+      List<software.amazon.cryptography.dynamoDbEncryption.model.SensitivePart> nativeValue) {
+    return software.amazon.dafny.conversion.ToDafny.Aggregate.GenericToSequence(
+        nativeValue, 
+        software.amazon.cryptography.dynamoDbEncryption.ToDafny::SensitivePart, 
+        SensitivePart._typeDescriptor());
+  }
+
+  public static DafnySequence<? extends CompoundBeacon> CompoundBeaconList(
+      List<software.amazon.cryptography.dynamoDbEncryption.model.CompoundBeacon> nativeValue) {
+    return software.amazon.dafny.conversion.ToDafny.Aggregate.GenericToSequence(
+        nativeValue, 
+        software.amazon.cryptography.dynamoDbEncryption.ToDafny::CompoundBeacon, 
+        CompoundBeacon._typeDescriptor());
+  }
+
+  public static DafnySequence<? extends Constructor> ConstructorList(
+      List<software.amazon.cryptography.dynamoDbEncryption.model.Constructor> nativeValue) {
+    return software.amazon.dafny.conversion.ToDafny.Aggregate.GenericToSequence(
+        nativeValue, 
+        software.amazon.cryptography.dynamoDbEncryption.ToDafny::Constructor, 
+        Constructor._typeDescriptor());
+  }
+
+  public static DafnySequence<? extends BeaconVersion> BeaconVersionList(
+      List<software.amazon.cryptography.dynamoDbEncryption.model.BeaconVersion> nativeValue) {
+    return software.amazon.dafny.conversion.ToDafny.Aggregate.GenericToSequence(
+        nativeValue, 
+        software.amazon.cryptography.dynamoDbEncryption.ToDafny::BeaconVersion, 
+        BeaconVersion._typeDescriptor());
+  }
+
+  public static DafnySequence<? extends ConstructorPart> ConstructorPartList(
+      List<software.amazon.cryptography.dynamoDbEncryption.model.ConstructorPart> nativeValue) {
+    return software.amazon.dafny.conversion.ToDafny.Aggregate.GenericToSequence(
+        nativeValue, 
+        software.amazon.cryptography.dynamoDbEncryption.ToDafny::ConstructorPart, 
+        ConstructorPart._typeDescriptor());
   }
 
   public static DafnyMap<? extends DafnySequence<? extends Character>, ? extends DynamoDbTableEncryptionConfig> DynamoDbTableEncryptionConfigs(
