DynamoDbEncryptionMiddlewareInternal/runtimes/java/src/main/smithy-generated/software/amazon/cryptography/dynamoDbEncryption/ToNative.java
@@ -11,6 +11,7 @@ import dafny.DafnyMap;
 import dafny.DafnySequence;
 import java.lang.Character;
 import java.lang.String;
+import java.util.List;
 import java.util.Map;
 import software.amazon.cryptography.dynamoDbEncryption.model.BatchExecuteStatementInputTransformInput;
 import software.amazon.cryptography.dynamoDbEncryption.model.BatchExecuteStatementInputTransformOutput;
@@ -24,11 +25,23 @@ import software.amazon.cryptography.dynamoDbEncryption.model.BatchWriteItemInput
 import software.amazon.cryptography.dynamoDbEncryption.model.BatchWriteItemInputTransformOutput;
 import software.amazon.cryptography.dynamoDbEncryption.model.BatchWriteItemOutputTransformInput;
 import software.amazon.cryptography.dynamoDbEncryption.model.BatchWriteItemOutputTransformOutput;
+import software.amazon.cryptography.dynamoDbEncryption.model.BeaconVersion;
 import software.amazon.cryptography.dynamoDbEncryption.model.CollectionOfErrors;
+import software.amazon.cryptography.dynamoDbEncryption.model.CompoundBeacon;
+import software.amazon.cryptography.dynamoDbEncryption.model.Constructor;
+import software.amazon.cryptography.dynamoDbEncryption.model.ConstructorPart;
+import software.amazon.cryptography.dynamoDbEncryption.model.CreateTableInputTransformInput;
+import software.amazon.cryptography.dynamoDbEncryption.model.CreateTableInputTransformOutput;
+import software.amazon.cryptography.dynamoDbEncryption.model.CreateTableOutputTransformInput;
+import software.amazon.cryptography.dynamoDbEncryption.model.CreateTableOutputTransformOutput;
 import software.amazon.cryptography.dynamoDbEncryption.model.DeleteItemInputTransformInput;
 import software.amazon.cryptography.dynamoDbEncryption.model.DeleteItemInputTransformOutput;
 import software.amazon.cryptography.dynamoDbEncryption.model.DeleteItemOutputTransformInput;
 import software.amazon.cryptography.dynamoDbEncryption.model.DeleteItemOutputTransformOutput;
+import software.amazon.cryptography.dynamoDbEncryption.model.DescribeTableInputTransformInput;
+import software.amazon.cryptography.dynamoDbEncryption.model.DescribeTableInputTransformOutput;
+import software.amazon.cryptography.dynamoDbEncryption.model.DescribeTableOutputTransformInput;
+import software.amazon.cryptography.dynamoDbEncryption.model.DescribeTableOutputTransformOutput;
 import software.amazon.cryptography.dynamoDbEncryption.model.DynamoDbEncryptionConfig;
 import software.amazon.cryptography.dynamoDbEncryption.model.DynamoDbEncryptionException;
 import software.amazon.cryptography.dynamoDbEncryption.model.DynamoDbTableEncryptionConfig;
@@ -45,6 +58,7 @@ import software.amazon.cryptography.dynamoDbEncryption.model.GetItemInputTransfo
 import software.amazon.cryptography.dynamoDbEncryption.model.GetItemOutputTransformInput;
 import software.amazon.cryptography.dynamoDbEncryption.model.GetItemOutputTransformOutput;
 import software.amazon.cryptography.dynamoDbEncryption.model.NativeError;
+import software.amazon.cryptography.dynamoDbEncryption.model.NonSensitivePart;
 import software.amazon.cryptography.dynamoDbEncryption.model.OpaqueError;
 import software.amazon.cryptography.dynamoDbEncryption.model.PutItemInputTransformInput;
 import software.amazon.cryptography.dynamoDbEncryption.model.PutItemInputTransformOutput;
@@ -58,6 +72,9 @@ import software.amazon.cryptography.dynamoDbEncryption.model.ScanInputTransformI
 import software.amazon.cryptography.dynamoDbEncryption.model.ScanInputTransformOutput;
 import software.amazon.cryptography.dynamoDbEncryption.model.ScanOutputTransformInput;
 import software.amazon.cryptography.dynamoDbEncryption.model.ScanOutputTransformOutput;
+import software.amazon.cryptography.dynamoDbEncryption.model.SearchConfig;
+import software.amazon.cryptography.dynamoDbEncryption.model.SensitivePart;
+import software.amazon.cryptography.dynamoDbEncryption.model.StandardBeacon;
 import software.amazon.cryptography.dynamoDbEncryption.model.TransactGetItemsInputTransformInput;
 import software.amazon.cryptography.dynamoDbEncryption.model.TransactGetItemsInputTransformOutput;
 import software.amazon.cryptography.dynamoDbEncryption.model.TransactGetItemsOutputTransformInput;
@@ -70,6 +87,11 @@ import software.amazon.cryptography.dynamoDbEncryption.model.UpdateItemInputTran
 import software.amazon.cryptography.dynamoDbEncryption.model.UpdateItemInputTransformOutput;
 import software.amazon.cryptography.dynamoDbEncryption.model.UpdateItemOutputTransformInput;
 import software.amazon.cryptography.dynamoDbEncryption.model.UpdateItemOutputTransformOutput;
+import software.amazon.cryptography.dynamoDbEncryption.model.UpdateTableInputTransformInput;
+import software.amazon.cryptography.dynamoDbEncryption.model.UpdateTableInputTransformOutput;
+import software.amazon.cryptography.dynamoDbEncryption.model.UpdateTableOutputTransformInput;
+import software.amazon.cryptography.dynamoDbEncryption.model.UpdateTableOutputTransformOutput;
+import software.amazon.cryptography.dynamoDbEncryption.model.VirtualField;
 
 public class ToNative {
   public static OpaqueError Error(Error_Opaque dafnyValue) {
@@ -108,12 +130,30 @@ public class ToNative {
     return nativeBuilder.build();
   }
 
+  public static TransactWriteItemsOutputTransformInput TransactWriteItemsOutputTransformInput(
+      Dafny.Aws.Cryptography.DynamoDbEncryption.Types.TransactWriteItemsOutputTransformInput dafnyValue) {
+    TransactWriteItemsOutputTransformInput.Builder nativeBuilder = TransactWriteItemsOutputTransformInput.builder();
+    nativeBuilder.sdkOutput(Dafny.Com.Amazonaws.Dynamodb.ToNative.TransactWriteItemsOutput(dafnyValue.dtor_sdkOutput()));
+    nativeBuilder.originalInput(Dafny.Com.Amazonaws.Dynamodb.ToNative.TransactWriteItemsInput(dafnyValue.dtor_originalInput()));
+    return nativeBuilder.build();
+  }
+
+  public static CreateTableInputTransformInput CreateTableInputTransformInput(
+      Dafny.Aws.Cryptography.DynamoDbEncryption.Types.CreateTableInputTransformInput dafnyValue) {
+    CreateTableInputTransformInput.Builder nativeBuilder = CreateTableInputTransformInput.builder();
+    nativeBuilder.sdkInput(Dafny.Com.Amazonaws.Dynamodb.ToNative.CreateTableInput(dafnyValue.dtor_sdkInput()));
+    return nativeBuilder.build();
+  }
+
   public static DynamoDbTableEncryptionConfig DynamoDbTableEncryptionConfig(
       Dafny.Aws.Cryptography.DynamoDbEncryption.Types.DynamoDbTableEncryptionConfig dafnyValue) {
     DynamoDbTableEncryptionConfig.Builder nativeBuilder = DynamoDbTableEncryptionConfig.builder();
     nativeBuilder.partitionKeyName(software.amazon.dafny.conversion.ToNative.Simple.String(dafnyValue.dtor_partitionKeyName()));
     if (dafnyValue.dtor_sortKeyName().is_Some()) {
       nativeBuilder.sortKeyName(software.amazon.dafny.conversion.ToNative.Simple.String(dafnyValue.dtor_sortKeyName().dtor_value()));
+    }
+    if (dafnyValue.dtor_beacons().is_Some()) {
+      nativeBuilder.beacons(ToNative.SearchConfig(dafnyValue.dtor_beacons().dtor_value()));
     }
     nativeBuilder.attributeActions(software.amazon.cryptography.dynamoDbItemEncryptor.ToNative.AttributeActions(dafnyValue.dtor_attributeActions()));
     if (dafnyValue.dtor_allowedUnauthenticatedAttributes().is_Some()) {
@@ -134,6 +174,20 @@ public class ToNative {
     return nativeBuilder.build();
   }
 
+  public static CreateTableOutputTransformOutput CreateTableOutputTransformOutput(
+      Dafny.Aws.Cryptography.DynamoDbEncryption.Types.CreateTableOutputTransformOutput dafnyValue) {
+    CreateTableOutputTransformOutput.Builder nativeBuilder = CreateTableOutputTransformOutput.builder();
+    nativeBuilder.transformedOutput(Dafny.Com.Amazonaws.Dynamodb.ToNative.CreateTableOutput(dafnyValue.dtor_transformedOutput()));
+    return nativeBuilder.build();
+  }
+
+  public static GetItemOutputTransformOutput GetItemOutputTransformOutput(
+      Dafny.Aws.Cryptography.DynamoDbEncryption.Types.GetItemOutputTransformOutput dafnyValue) {
+    GetItemOutputTransformOutput.Builder nativeBuilder = GetItemOutputTransformOutput.builder();
+    nativeBuilder.transformedOutput(Dafny.Com.Amazonaws.Dynamodb.ToNative.GetItemOutput(dafnyValue.dtor_transformedOutput()));
+    return nativeBuilder.build();
+  }
+
   public static PutItemInputTransformInput PutItemInputTransformInput(
       Dafny.Aws.Cryptography.DynamoDbEncryption.Types.PutItemInputTransformInput dafnyValue) {
     PutItemInputTransformInput.Builder nativeBuilder = PutItemInputTransformInput.builder();
@@ -141,11 +195,83 @@ public class ToNative {
     return nativeBuilder.build();
   }
 
-  public static TransactWriteItemsOutputTransformInput TransactWriteItemsOutputTransformInput(
-      Dafny.Aws.Cryptography.DynamoDbEncryption.Types.TransactWriteItemsOutputTransformInput dafnyValue) {
-    TransactWriteItemsOutputTransformInput.Builder nativeBuilder = TransactWriteItemsOutputTransformInput.builder();
-    nativeBuilder.sdkOutput(Dafny.Com.Amazonaws.Dynamodb.ToNative.TransactWriteItemsOutput(dafnyValue.dtor_sdkOutput()));
-    nativeBuilder.originalInput(Dafny.Com.Amazonaws.Dynamodb.ToNative.TransactWriteItemsInput(dafnyValue.dtor_originalInput()));
+  public static NonSensitivePart NonSensitivePart(
+      Dafny.Aws.Cryptography.DynamoDbEncryption.Types.NonSensitivePart dafnyValue) {
+    NonSensitivePart.Builder nativeBuilder = NonSensitivePart.builder();
+    nativeBuilder.name(software.amazon.dafny.conversion.ToNative.Simple.String(dafnyValue.dtor_name()));
+    nativeBuilder.loc(software.amazon.dafny.conversion.ToNative.Simple.String(dafnyValue.dtor_loc()));
+    return nativeBuilder.build();
+  }
+
+  public static TransactGetItemsInputTransformOutput TransactGetItemsInputTransformOutput(
+      Dafny.Aws.Cryptography.DynamoDbEncryption.Types.TransactGetItemsInputTransformOutput dafnyValue) {
+    TransactGetItemsInputTransformOutput.Builder nativeBuilder = TransactGetItemsInputTransformOutput.builder();
+    nativeBuilder.transformedInput(Dafny.Com.Amazonaws.Dynamodb.ToNative.TransactGetItemsInput(dafnyValue.dtor_transformedInput()));
+    return nativeBuilder.build();
+  }
+
+  public static QueryInputTransformOutput QueryInputTransformOutput(
+      Dafny.Aws.Cryptography.DynamoDbEncryption.Types.QueryInputTransformOutput dafnyValue) {
+    QueryInputTransformOutput.Builder nativeBuilder = QueryInputTransformOutput.builder();
+    nativeBuilder.transformedInput(Dafny.Com.Amazonaws.Dynamodb.ToNative.QueryInput(dafnyValue.dtor_transformedInput()));
+    return nativeBuilder.build();
+  }
+
+  public static GetItemInputTransformOutput GetItemInputTransformOutput(
+      Dafny.Aws.Cryptography.DynamoDbEncryption.Types.GetItemInputTransformOutput dafnyValue) {
+    GetItemInputTransformOutput.Builder nativeBuilder = GetItemInputTransformOutput.builder();
+    nativeBuilder.transformedInput(Dafny.Com.Amazonaws.Dynamodb.ToNative.GetItemInput(dafnyValue.dtor_transformedInput()));
+    return nativeBuilder.build();
+  }
+
+  public static ExecuteTransactionInputTransformOutput ExecuteTransactionInputTransformOutput(
+      Dafny.Aws.Cryptography.DynamoDbEncryption.Types.ExecuteTransactionInputTransformOutput dafnyValue) {
+    ExecuteTransactionInputTransformOutput.Builder nativeBuilder = ExecuteTransactionInputTransformOutput.builder();
+    nativeBuilder.transformedInput(Dafny.Com.Amazonaws.Dynamodb.ToNative.ExecuteTransactionInput(dafnyValue.dtor_transformedInput()));
+    return nativeBuilder.build();
+  }
+
+  public static ExecuteStatementInputTransformInput ExecuteStatementInputTransformInput(
+      Dafny.Aws.Cryptography.DynamoDbEncryption.Types.ExecuteStatementInputTransformInput dafnyValue) {
+    ExecuteStatementInputTransformInput.Builder nativeBuilder = ExecuteStatementInputTransformInput.builder();
+    nativeBuilder.sdkInput(Dafny.Com.Amazonaws.Dynamodb.ToNative.ExecuteStatementInput(dafnyValue.dtor_sdkInput()));
+    return nativeBuilder.build();
+  }
+
+  public static BatchExecuteStatementInputTransformInput BatchExecuteStatementInputTransformInput(
+      Dafny.Aws.Cryptography.DynamoDbEncryption.Types.BatchExecuteStatementInputTransformInput dafnyValue) {
+    BatchExecuteStatementInputTransformInput.Builder nativeBuilder = BatchExecuteStatementInputTransformInput.builder();
+    nativeBuilder.sdkInput(Dafny.Com.Amazonaws.Dynamodb.ToNative.BatchExecuteStatementInput(dafnyValue.dtor_sdkInput()));
+    return nativeBuilder.build();
+  }
+
+  public static TransactGetItemsOutputTransformOutput TransactGetItemsOutputTransformOutput(
+      Dafny.Aws.Cryptography.DynamoDbEncryption.Types.TransactGetItemsOutputTransformOutput dafnyValue) {
+    TransactGetItemsOutputTransformOutput.Builder nativeBuilder = TransactGetItemsOutputTransformOutput.builder();
+    nativeBuilder.transformedOutput(Dafny.Com.Amazonaws.Dynamodb.ToNative.TransactGetItemsOutput(dafnyValue.dtor_transformedOutput()));
+    return nativeBuilder.build();
+  }
+
+  public static SearchConfig SearchConfig(
+      Dafny.Aws.Cryptography.DynamoDbEncryption.Types.SearchConfig dafnyValue) {
+    SearchConfig.Builder nativeBuilder = SearchConfig.builder();
+    nativeBuilder.versions(ToNative.BeaconVersionList(dafnyValue.dtor_versions()));
+    nativeBuilder.writeVersion((dafnyValue.dtor_writeVersion()));
+    return nativeBuilder.build();
+  }
+
+  public static VirtualField VirtualField(
+      Dafny.Aws.Cryptography.DynamoDbEncryption.Types.VirtualField dafnyValue) {
+    VirtualField.Builder nativeBuilder = VirtualField.builder();
+    nativeBuilder.name(software.amazon.dafny.conversion.ToNative.Simple.String(dafnyValue.dtor_name()));
+    nativeBuilder.config(software.amazon.dafny.conversion.ToNative.Simple.String(dafnyValue.dtor_config()));
+    return nativeBuilder.build();
+  }
+
+  public static PutItemInputTransformOutput PutItemInputTransformOutput(
+      Dafny.Aws.Cryptography.DynamoDbEncryption.Types.PutItemInputTransformOutput dafnyValue) {
+    PutItemInputTransformOutput.Builder nativeBuilder = PutItemInputTransformOutput.builder();
+    nativeBuilder.transformedInput(Dafny.Com.Amazonaws.Dynamodb.ToNative.PutItemInput(dafnyValue.dtor_transformedInput()));
     return nativeBuilder.build();
   }
 
@@ -157,39 +283,53 @@ public class ToNative {
     return nativeBuilder.build();
   }
 
-  public static DeleteItemOutputTransformInput DeleteItemOutputTransformInput(
-      Dafny.Aws.Cryptography.DynamoDbEncryption.Types.DeleteItemOutputTransformInput dafnyValue) {
-    DeleteItemOutputTransformInput.Builder nativeBuilder = DeleteItemOutputTransformInput.builder();
-    nativeBuilder.sdkOutput(Dafny.Com.Amazonaws.Dynamodb.ToNative.DeleteItemOutput(dafnyValue.dtor_sdkOutput()));
-    nativeBuilder.originalInput(Dafny.Com.Amazonaws.Dynamodb.ToNative.DeleteItemInput(dafnyValue.dtor_originalInput()));
+  public static DeleteItemInputTransformInput DeleteItemInputTransformInput(
+      Dafny.Aws.Cryptography.DynamoDbEncryption.Types.DeleteItemInputTransformInput dafnyValue) {
+    DeleteItemInputTransformInput.Builder nativeBuilder = DeleteItemInputTransformInput.builder();
+    nativeBuilder.sdkInput(Dafny.Com.Amazonaws.Dynamodb.ToNative.DeleteItemInput(dafnyValue.dtor_sdkInput()));
     return nativeBuilder.build();
   }
 
-  public static BatchExecuteStatementInputTransformInput BatchExecuteStatementInputTransformInput(
-      Dafny.Aws.Cryptography.DynamoDbEncryption.Types.BatchExecuteStatementInputTransformInput dafnyValue) {
-    BatchExecuteStatementInputTransformInput.Builder nativeBuilder = BatchExecuteStatementInputTransformInput.builder();
-    nativeBuilder.sdkInput(Dafny.Com.Amazonaws.Dynamodb.ToNative.BatchExecuteStatementInput(dafnyValue.dtor_sdkInput()));
+  public static QueryOutputTransformInput QueryOutputTransformInput(
+      Dafny.Aws.Cryptography.DynamoDbEncryption.Types.QueryOutputTransformInput dafnyValue) {
+    QueryOutputTransformInput.Builder nativeBuilder = QueryOutputTransformInput.builder();
+    nativeBuilder.sdkOutput(Dafny.Com.Amazonaws.Dynamodb.ToNative.QueryOutput(dafnyValue.dtor_sdkOutput()));
+    nativeBuilder.originalInput(Dafny.Com.Amazonaws.Dynamodb.ToNative.QueryInput(dafnyValue.dtor_originalInput()));
     return nativeBuilder.build();
   }
 
-  public static ExecuteStatementInputTransformOutput ExecuteStatementInputTransformOutput(
-      Dafny.Aws.Cryptography.DynamoDbEncryption.Types.ExecuteStatementInputTransformOutput dafnyValue) {
-    ExecuteStatementInputTransformOutput.Builder nativeBuilder = ExecuteStatementInputTransformOutput.builder();
-    nativeBuilder.transformedInput(Dafny.Com.Amazonaws.Dynamodb.ToNative.ExecuteStatementInput(dafnyValue.dtor_transformedInput()));
+  public static GetItemInputTransformInput GetItemInputTransformInput(
+      Dafny.Aws.Cryptography.DynamoDbEncryption.Types.GetItemInputTransformInput dafnyValue) {
+    GetItemInputTransformInput.Builder nativeBuilder = GetItemInputTransformInput.builder();
+    nativeBuilder.sdkInput(Dafny.Com.Amazonaws.Dynamodb.ToNative.GetItemInput(dafnyValue.dtor_sdkInput()));
     return nativeBuilder.build();
   }
 
-  public static GetItemOutputTransformOutput GetItemOutputTransformOutput(
-      Dafny.Aws.Cryptography.DynamoDbEncryption.Types.GetItemOutputTransformOutput dafnyValue) {
-    GetItemOutputTransformOutput.Builder nativeBuilder = GetItemOutputTransformOutput.builder();
-    nativeBuilder.transformedOutput(Dafny.Com.Amazonaws.Dynamodb.ToNative.GetItemOutput(dafnyValue.dtor_transformedOutput()));
+  public static DescribeTableInputTransformInput DescribeTableInputTransformInput(
+      Dafny.Aws.Cryptography.DynamoDbEncryption.Types.DescribeTableInputTransformInput dafnyValue) {
+    DescribeTableInputTransformInput.Builder nativeBuilder = DescribeTableInputTransformInput.builder();
+    nativeBuilder.sdkInput(Dafny.Com.Amazonaws.Dynamodb.ToNative.DescribeTableInput(dafnyValue.dtor_sdkInput()));
     return nativeBuilder.build();
   }
 
-  public static BatchGetItemOutputTransformOutput BatchGetItemOutputTransformOutput(
-      Dafny.Aws.Cryptography.DynamoDbEncryption.Types.BatchGetItemOutputTransformOutput dafnyValue) {
-    BatchGetItemOutputTransformOutput.Builder nativeBuilder = BatchGetItemOutputTransformOutput.builder();
-    nativeBuilder.transformedOutput(Dafny.Com.Amazonaws.Dynamodb.ToNative.BatchGetItemOutput(dafnyValue.dtor_transformedOutput()));
+  public static ScanInputTransformInput ScanInputTransformInput(
+      Dafny.Aws.Cryptography.DynamoDbEncryption.Types.ScanInputTransformInput dafnyValue) {
+    ScanInputTransformInput.Builder nativeBuilder = ScanInputTransformInput.builder();
+    nativeBuilder.sdkInput(Dafny.Com.Amazonaws.Dynamodb.ToNative.ScanInput(dafnyValue.dtor_sdkInput()));
+    return nativeBuilder.build();
+  }
+
+  public static UpdateTableOutputTransformOutput UpdateTableOutputTransformOutput(
+      Dafny.Aws.Cryptography.DynamoDbEncryption.Types.UpdateTableOutputTransformOutput dafnyValue) {
+    UpdateTableOutputTransformOutput.Builder nativeBuilder = UpdateTableOutputTransformOutput.builder();
+    nativeBuilder.transformedOutput(Dafny.Com.Amazonaws.Dynamodb.ToNative.UpdateTableOutput(dafnyValue.dtor_transformedOutput()));
+    return nativeBuilder.build();
+  }
+
+  public static DescribeTableOutputTransformOutput DescribeTableOutputTransformOutput(
+      Dafny.Aws.Cryptography.DynamoDbEncryption.Types.DescribeTableOutputTransformOutput dafnyValue) {
+    DescribeTableOutputTransformOutput.Builder nativeBuilder = DescribeTableOutputTransformOutput.builder();
+    nativeBuilder.transformedOutput(Dafny.Com.Amazonaws.Dynamodb.ToNative.DescribeTableOutput(dafnyValue.dtor_transformedOutput()));
     return nativeBuilder.build();
   }
 
@@ -200,25 +340,43 @@ public class ToNative {
     return nativeBuilder.build();
   }
 
-  public static DeleteItemInputTransformOutput DeleteItemInputTransformOutput(
-      Dafny.Aws.Cryptography.DynamoDbEncryption.Types.DeleteItemInputTransformOutput dafnyValue) {
-    DeleteItemInputTransformOutput.Builder nativeBuilder = DeleteItemInputTransformOutput.builder();
-    nativeBuilder.transformedInput(Dafny.Com.Amazonaws.Dynamodb.ToNative.DeleteItemInput(dafnyValue.dtor_transformedInput()));
+  public static GetItemOutputTransformInput GetItemOutputTransformInput(
+      Dafny.Aws.Cryptography.DynamoDbEncryption.Types.GetItemOutputTransformInput dafnyValue) {
+    GetItemOutputTransformInput.Builder nativeBuilder = GetItemOutputTransformInput.builder();
+    nativeBuilder.sdkOutput(Dafny.Com.Amazonaws.Dynamodb.ToNative.GetItemOutput(dafnyValue.dtor_sdkOutput()));
+    nativeBuilder.originalInput(Dafny.Com.Amazonaws.Dynamodb.ToNative.GetItemInput(dafnyValue.dtor_originalInput()));
     return nativeBuilder.build();
   }
 
-  public static UpdateItemOutputTransformOutput UpdateItemOutputTransformOutput(
-      Dafny.Aws.Cryptography.DynamoDbEncryption.Types.UpdateItemOutputTransformOutput dafnyValue) {
-    UpdateItemOutputTransformOutput.Builder nativeBuilder = UpdateItemOutputTransformOutput.builder();
-    nativeBuilder.transformedOutput(Dafny.Com.Amazonaws.Dynamodb.ToNative.UpdateItemOutput(dafnyValue.dtor_transformedOutput()));
+  public static TransactWriteItemsInputTransformOutput TransactWriteItemsInputTransformOutput(
+      Dafny.Aws.Cryptography.DynamoDbEncryption.Types.TransactWriteItemsInputTransformOutput dafnyValue) {
+    TransactWriteItemsInputTransformOutput.Builder nativeBuilder = TransactWriteItemsInputTransformOutput.builder();
+    nativeBuilder.transformedInput(Dafny.Com.Amazonaws.Dynamodb.ToNative.TransactWriteItemsInput(dafnyValue.dtor_transformedInput()));
     return nativeBuilder.build();
   }
 
-  public static PutItemOutputTransformInput PutItemOutputTransformInput(
-      Dafny.Aws.Cryptography.DynamoDbEncryption.Types.PutItemOutputTransformInput dafnyValue) {
-    PutItemOutputTransformInput.Builder nativeBuilder = PutItemOutputTransformInput.builder();
-    nativeBuilder.sdkOutput(Dafny.Com.Amazonaws.Dynamodb.ToNative.PutItemOutput(dafnyValue.dtor_sdkOutput()));
-    nativeBuilder.originalInput(Dafny.Com.Amazonaws.Dynamodb.ToNative.PutItemInput(dafnyValue.dtor_originalInput()));
+  public static BatchGetItemOutputTransformInput BatchGetItemOutputTransformInput(
+      Dafny.Aws.Cryptography.DynamoDbEncryption.Types.BatchGetItemOutputTransformInput dafnyValue) {
+    BatchGetItemOutputTransformInput.Builder nativeBuilder = BatchGetItemOutputTransformInput.builder();
+    nativeBuilder.sdkOutput(Dafny.Com.Amazonaws.Dynamodb.ToNative.BatchGetItemOutput(dafnyValue.dtor_sdkOutput()));
+    nativeBuilder.originalInput(Dafny.Com.Amazonaws.Dynamodb.ToNative.BatchGetItemInput(dafnyValue.dtor_originalInput()));
+    return nativeBuilder.build();
+  }
+
+  public static BeaconVersion BeaconVersion(
+      Dafny.Aws.Cryptography.DynamoDbEncryption.Types.BeaconVersion dafnyValue) {
+    BeaconVersion.Builder nativeBuilder = BeaconVersion.builder();
+    nativeBuilder.version((dafnyValue.dtor_version()));
+    nativeBuilder.keyring(software.amazon.cryptography.materialProviders.ToNative.Keyring(dafnyValue.dtor_keyring()));
+    if (dafnyValue.dtor_standardBeacons().is_Some()) {
+      nativeBuilder.standardBeacons(ToNative.StandardBeaconList(dafnyValue.dtor_standardBeacons().dtor_value()));
+    }
+    if (dafnyValue.dtor_compoundBeacons().is_Some()) {
+      nativeBuilder.compoundBeacons(ToNative.CompoundBeaconList(dafnyValue.dtor_compoundBeacons().dtor_value()));
+    }
+    if (dafnyValue.dtor_virtualFields().is_Some()) {
+      nativeBuilder.virtualFields(ToNative.VirtualFieldList(dafnyValue.dtor_virtualFields().dtor_value()));
+    }
     return nativeBuilder.build();
   }
 
@@ -237,90 +395,47 @@ public class ToNative {
     return nativeBuilder.build();
   }
 
-  public static PutItemInputTransformOutput PutItemInputTransformOutput(
-      Dafny.Aws.Cryptography.DynamoDbEncryption.Types.PutItemInputTransformOutput dafnyValue) {
-    PutItemInputTransformOutput.Builder nativeBuilder = PutItemInputTransformOutput.builder();
-    nativeBuilder.transformedInput(Dafny.Com.Amazonaws.Dynamodb.ToNative.PutItemInput(dafnyValue.dtor_transformedInput()));
+  public static DeleteItemOutputTransformInput DeleteItemOutputTransformInput(
+      Dafny.Aws.Cryptography.DynamoDbEncryption.Types.DeleteItemOutputTransformInput dafnyValue) {
+    DeleteItemOutputTransformInput.Builder nativeBuilder = DeleteItemOutputTransformInput.builder();
+    nativeBuilder.sdkOutput(Dafny.Com.Amazonaws.Dynamodb.ToNative.DeleteItemOutput(dafnyValue.dtor_sdkOutput()));
+    nativeBuilder.originalInput(Dafny.Com.Amazonaws.Dynamodb.ToNative.DeleteItemInput(dafnyValue.dtor_originalInput()));
     return nativeBuilder.build();
   }
 
-  public static BatchGetItemOutputTransformInput BatchGetItemOutputTransformInput(
-      Dafny.Aws.Cryptography.DynamoDbEncryption.Types.BatchGetItemOutputTransformInput dafnyValue) {
-    BatchGetItemOutputTransformInput.Builder nativeBuilder = BatchGetItemOutputTransformInput.builder();
-    nativeBuilder.sdkOutput(Dafny.Com.Amazonaws.Dynamodb.ToNative.BatchGetItemOutput(dafnyValue.dtor_sdkOutput()));
-    nativeBuilder.originalInput(Dafny.Com.Amazonaws.Dynamodb.ToNative.BatchGetItemInput(dafnyValue.dtor_originalInput()));
+  public static DynamoDbEncryptionConfig DynamoDbEncryptionConfig(
+      Dafny.Aws.Cryptography.DynamoDbEncryption.Types.DynamoDbEncryptionConfig dafnyValue) {
+    DynamoDbEncryptionConfig.Builder nativeBuilder = DynamoDbEncryptionConfig.builder();
+    nativeBuilder.tableEncryptionConfigs(ToNative.DynamoDbTableEncryptionConfigs(dafnyValue.dtor_tableEncryptionConfigs()));
     return nativeBuilder.build();
   }
 
-  public static QueryOutputTransformInput QueryOutputTransformInput(
-      Dafny.Aws.Cryptography.DynamoDbEncryption.Types.QueryOutputTransformInput dafnyValue) {
-    QueryOutputTransformInput.Builder nativeBuilder = QueryOutputTransformInput.builder();
-    nativeBuilder.sdkOutput(Dafny.Com.Amazonaws.Dynamodb.ToNative.QueryOutput(dafnyValue.dtor_sdkOutput()));
-    nativeBuilder.originalInput(Dafny.Com.Amazonaws.Dynamodb.ToNative.QueryInput(dafnyValue.dtor_originalInput()));
+  public static BatchExecuteStatementInputTransformOutput BatchExecuteStatementInputTransformOutput(
+      Dafny.Aws.Cryptography.DynamoDbEncryption.Types.BatchExecuteStatementInputTransformOutput dafnyValue) {
+    BatchExecuteStatementInputTransformOutput.Builder nativeBuilder = BatchExecuteStatementInputTransformOutput.builder();
+    nativeBuilder.transformedInput(Dafny.Com.Amazonaws.Dynamodb.ToNative.BatchExecuteStatementInput(dafnyValue.dtor_transformedInput()));
     return nativeBuilder.build();
   }
 
-  public static DeleteItemInputTransformInput DeleteItemInputTransformInput(
-      Dafny.Aws.Cryptography.DynamoDbEncryption.Types.DeleteItemInputTransformInput dafnyValue) {
-    DeleteItemInputTransformInput.Builder nativeBuilder = DeleteItemInputTransformInput.builder();
-    nativeBuilder.sdkInput(Dafny.Com.Amazonaws.Dynamodb.ToNative.DeleteItemInput(dafnyValue.dtor_sdkInput()));
+  public static UpdateItemOutputTransformOutput UpdateItemOutputTransformOutput(
+      Dafny.Aws.Cryptography.DynamoDbEncryption.Types.UpdateItemOutputTransformOutput dafnyValue) {
+    UpdateItemOutputTransformOutput.Builder nativeBuilder = UpdateItemOutputTransformOutput.builder();
+    nativeBuilder.transformedOutput(Dafny.Com.Amazonaws.Dynamodb.ToNative.UpdateItemOutput(dafnyValue.dtor_transformedOutput()));
     return nativeBuilder.build();
   }
 
-  public static TransactWriteItemsInputTransformOutput TransactWriteItemsInputTransformOutput(
-      Dafny.Aws.Cryptography.DynamoDbEncryption.Types.TransactWriteItemsInputTransformOutput dafnyValue) {
-    TransactWriteItemsInputTransformOutput.Builder nativeBuilder = TransactWriteItemsInputTransformOutput.builder();
-    nativeBuilder.transformedInput(Dafny.Com.Amazonaws.Dynamodb.ToNative.TransactWriteItemsInput(dafnyValue.dtor_transformedInput()));
+  public static DeleteItemInputTransformOutput DeleteItemInputTransformOutput(
+      Dafny.Aws.Cryptography.DynamoDbEncryption.Types.DeleteItemInputTransformOutput dafnyValue) {
+    DeleteItemInputTransformOutput.Builder nativeBuilder = DeleteItemInputTransformOutput.builder();
+    nativeBuilder.transformedInput(Dafny.Com.Amazonaws.Dynamodb.ToNative.DeleteItemInput(dafnyValue.dtor_transformedInput()));
     return nativeBuilder.build();
   }
 
-  public static GetItemInputTransformOutput GetItemInputTransformOutput(
-      Dafny.Aws.Cryptography.DynamoDbEncryption.Types.GetItemInputTransformOutput dafnyValue) {
-    GetItemInputTransformOutput.Builder nativeBuilder = GetItemInputTransformOutput.builder();
-    nativeBuilder.transformedInput(Dafny.Com.Amazonaws.Dynamodb.ToNative.GetItemInput(dafnyValue.dtor_transformedInput()));
-    return nativeBuilder.build();
-  }
-
-  public static GetItemInputTransformInput GetItemInputTransformInput(
-      Dafny.Aws.Cryptography.DynamoDbEncryption.Types.GetItemInputTransformInput dafnyValue) {
-    GetItemInputTransformInput.Builder nativeBuilder = GetItemInputTransformInput.builder();
-    nativeBuilder.sdkInput(Dafny.Com.Amazonaws.Dynamodb.ToNative.GetItemInput(dafnyValue.dtor_sdkInput()));
-    return nativeBuilder.build();
-  }
-
-  public static QueryInputTransformOutput QueryInputTransformOutput(
-      Dafny.Aws.Cryptography.DynamoDbEncryption.Types.QueryInputTransformOutput dafnyValue) {
-    QueryInputTransformOutput.Builder nativeBuilder = QueryInputTransformOutput.builder();
-    nativeBuilder.transformedInput(Dafny.Com.Amazonaws.Dynamodb.ToNative.QueryInput(dafnyValue.dtor_transformedInput()));
-    return nativeBuilder.build();
-  }
-
-  public static BatchWriteItemOutputTransformOutput BatchWriteItemOutputTransformOutput(
-      Dafny.Aws.Cryptography.DynamoDbEncryption.Types.BatchWriteItemOutputTransformOutput dafnyValue) {
-    BatchWriteItemOutputTransformOutput.Builder nativeBuilder = BatchWriteItemOutputTransformOutput.builder();
-    nativeBuilder.transformedOutput(Dafny.Com.Amazonaws.Dynamodb.ToNative.BatchWriteItemOutput(dafnyValue.dtor_transformedOutput()));
-    return nativeBuilder.build();
-  }
-
-  public static GetItemOutputTransformInput GetItemOutputTransformInput(
-      Dafny.Aws.Cryptography.DynamoDbEncryption.Types.GetItemOutputTransformInput dafnyValue) {
-    GetItemOutputTransformInput.Builder nativeBuilder = GetItemOutputTransformInput.builder();
-    nativeBuilder.sdkOutput(Dafny.Com.Amazonaws.Dynamodb.ToNative.GetItemOutput(dafnyValue.dtor_sdkOutput()));
-    nativeBuilder.originalInput(Dafny.Com.Amazonaws.Dynamodb.ToNative.GetItemInput(dafnyValue.dtor_originalInput()));
-    return nativeBuilder.build();
-  }
-
-  public static PutItemOutputTransformOutput PutItemOutputTransformOutput(
-      Dafny.Aws.Cryptography.DynamoDbEncryption.Types.PutItemOutputTransformOutput dafnyValue) {
-    PutItemOutputTransformOutput.Builder nativeBuilder = PutItemOutputTransformOutput.builder();
-    nativeBuilder.transformedOutput(Dafny.Com.Amazonaws.Dynamodb.ToNative.PutItemOutput(dafnyValue.dtor_transformedOutput()));
-    return nativeBuilder.build();
-  }
-
-  public static ExecuteTransactionOutputTransformOutput ExecuteTransactionOutputTransformOutput(
-      Dafny.Aws.Cryptography.DynamoDbEncryption.Types.ExecuteTransactionOutputTransformOutput dafnyValue) {
-    ExecuteTransactionOutputTransformOutput.Builder nativeBuilder = ExecuteTransactionOutputTransformOutput.builder();
-    nativeBuilder.transformedOutput(Dafny.Com.Amazonaws.Dynamodb.ToNative.ExecuteTransactionOutput(dafnyValue.dtor_transformedOutput()));
+  public static UpdateTableOutputTransformInput UpdateTableOutputTransformInput(
+      Dafny.Aws.Cryptography.DynamoDbEncryption.Types.UpdateTableOutputTransformInput dafnyValue) {
+    UpdateTableOutputTransformInput.Builder nativeBuilder = UpdateTableOutputTransformInput.builder();
+    nativeBuilder.sdkOutput(Dafny.Com.Amazonaws.Dynamodb.ToNative.UpdateTableOutput(dafnyValue.dtor_sdkOutput()));
+    nativeBuilder.originalInput(Dafny.Com.Amazonaws.Dynamodb.ToNative.UpdateTableInput(dafnyValue.dtor_originalInput()));
     return nativeBuilder.build();
   }
 
@@ -331,6 +446,74 @@ public class ToNative {
     return nativeBuilder.build();
   }
 
+  public static UpdateItemInputTransformOutput UpdateItemInputTransformOutput(
+      Dafny.Aws.Cryptography.DynamoDbEncryption.Types.UpdateItemInputTransformOutput dafnyValue) {
+    UpdateItemInputTransformOutput.Builder nativeBuilder = UpdateItemInputTransformOutput.builder();
+    nativeBuilder.transformedInput(Dafny.Com.Amazonaws.Dynamodb.ToNative.UpdateItemInput(dafnyValue.dtor_transformedInput()));
+    return nativeBuilder.build();
+  }
+
+  public static StandardBeacon StandardBeacon(
+      Dafny.Aws.Cryptography.DynamoDbEncryption.Types.StandardBeacon dafnyValue) {
+    StandardBeacon.Builder nativeBuilder = StandardBeacon.builder();
+    nativeBuilder.name(software.amazon.dafny.conversion.ToNative.Simple.String(dafnyValue.dtor_name()));
+    nativeBuilder.length((dafnyValue.dtor_length()));
+    nativeBuilder.loc(software.amazon.dafny.conversion.ToNative.Simple.String(dafnyValue.dtor_loc()));
+    return nativeBuilder.build();
+  }
+
+  public static ExecuteTransactionOutputTransformOutput ExecuteTransactionOutputTransformOutput(
+      Dafny.Aws.Cryptography.DynamoDbEncryption.Types.ExecuteTransactionOutputTransformOutput dafnyValue) {
+    ExecuteTransactionOutputTransformOutput.Builder nativeBuilder = ExecuteTransactionOutputTransformOutput.builder();
+    nativeBuilder.transformedOutput(Dafny.Com.Amazonaws.Dynamodb.ToNative.ExecuteTransactionOutput(dafnyValue.dtor_transformedOutput()));
+    return nativeBuilder.build();
+  }
+
+  public static SensitivePart SensitivePart(
+      Dafny.Aws.Cryptography.DynamoDbEncryption.Types.SensitivePart dafnyValue) {
+    SensitivePart.Builder nativeBuilder = SensitivePart.builder();
+    nativeBuilder.name(software.amazon.dafny.conversion.ToNative.Simple.String(dafnyValue.dtor_name()));
+    nativeBuilder.length((dafnyValue.dtor_length()));
+    nativeBuilder.loc(software.amazon.dafny.conversion.ToNative.Simple.String(dafnyValue.dtor_loc()));
+    return nativeBuilder.build();
+  }
+
+  public static Constructor Constructor(
+      Dafny.Aws.Cryptography.DynamoDbEncryption.Types.Constructor dafnyValue) {
+    Constructor.Builder nativeBuilder = Constructor.builder();
+    nativeBuilder.parts(ToNative.ConstructorPartList(dafnyValue.dtor_parts()));
+    return nativeBuilder.build();
+  }
+
+  public static ConstructorPart ConstructorPart(
+      Dafny.Aws.Cryptography.DynamoDbEncryption.Types.ConstructorPart dafnyValue) {
+    ConstructorPart.Builder nativeBuilder = ConstructorPart.builder();
+    nativeBuilder.name(software.amazon.dafny.conversion.ToNative.Simple.String(dafnyValue.dtor_name()));
+    nativeBuilder.required((dafnyValue.dtor_required()));
+    return nativeBuilder.build();
+  }
+
+  public static UpdateTableInputTransformInput UpdateTableInputTransformInput(
+      Dafny.Aws.Cryptography.DynamoDbEncryption.Types.UpdateTableInputTransformInput dafnyValue) {
+    UpdateTableInputTransformInput.Builder nativeBuilder = UpdateTableInputTransformInput.builder();
+    nativeBuilder.sdkInput(Dafny.Com.Amazonaws.Dynamodb.ToNative.UpdateTableInput(dafnyValue.dtor_sdkInput()));
+    return nativeBuilder.build();
+  }
+
+  public static TransactGetItemsInputTransformInput TransactGetItemsInputTransformInput(
+      Dafny.Aws.Cryptography.DynamoDbEncryption.Types.TransactGetItemsInputTransformInput dafnyValue) {
+    TransactGetItemsInputTransformInput.Builder nativeBuilder = TransactGetItemsInputTransformInput.builder();
+    nativeBuilder.sdkInput(Dafny.Com.Amazonaws.Dynamodb.ToNative.TransactGetItemsInput(dafnyValue.dtor_sdkInput()));
+    return nativeBuilder.build();
+  }
+
+  public static PutItemOutputTransformOutput PutItemOutputTransformOutput(
+      Dafny.Aws.Cryptography.DynamoDbEncryption.Types.PutItemOutputTransformOutput dafnyValue) {
+    PutItemOutputTransformOutput.Builder nativeBuilder = PutItemOutputTransformOutput.builder();
+    nativeBuilder.transformedOutput(Dafny.Com.Amazonaws.Dynamodb.ToNative.PutItemOutput(dafnyValue.dtor_transformedOutput()));
+    return nativeBuilder.build();
+  }
+
   public static QueryOutputTransformOutput QueryOutputTransformOutput(
       Dafny.Aws.Cryptography.DynamoDbEncryption.Types.QueryOutputTransformOutput dafnyValue) {
     QueryOutputTransformOutput.Builder nativeBuilder = QueryOutputTransformOutput.builder();
@@ -338,10 +521,39 @@ public class ToNative {
     return nativeBuilder.build();
   }
 
-  public static BatchExecuteStatementInputTransformOutput BatchExecuteStatementInputTransformOutput(
-      Dafny.Aws.Cryptography.DynamoDbEncryption.Types.BatchExecuteStatementInputTransformOutput dafnyValue) {
-    BatchExecuteStatementInputTransformOutput.Builder nativeBuilder = BatchExecuteStatementInputTransformOutput.builder();
-    nativeBuilder.transformedInput(Dafny.Com.Amazonaws.Dynamodb.ToNative.BatchExecuteStatementInput(dafnyValue.dtor_transformedInput()));
+  public static UpdateItemInputTransformInput UpdateItemInputTransformInput(
+      Dafny.Aws.Cryptography.DynamoDbEncryption.Types.UpdateItemInputTransformInput dafnyValue) {
+    UpdateItemInputTransformInput.Builder nativeBuilder = UpdateItemInputTransformInput.builder();
+    nativeBuilder.sdkInput(Dafny.Com.Amazonaws.Dynamodb.ToNative.UpdateItemInput(dafnyValue.dtor_sdkInput()));
+    return nativeBuilder.build();
+  }
+
+  public static CompoundBeacon CompoundBeacon(
+      Dafny.Aws.Cryptography.DynamoDbEncryption.Types.CompoundBeacon dafnyValue) {
+    CompoundBeacon.Builder nativeBuilder = CompoundBeacon.builder();
+    nativeBuilder.name(software.amazon.dafny.conversion.ToNative.Simple.String(dafnyValue.dtor_name()));
+    nativeBuilder.split(software.amazon.dafny.conversion.ToNative.Simple.String(dafnyValue.dtor_split()));
+    nativeBuilder.sensitive(ToNative.SensitivePartsList(dafnyValue.dtor_sensitive()));
+    if (dafnyValue.dtor_nonSensitive().is_Some()) {
+      nativeBuilder.nonSensitive(ToNative.NonSensitivePartsList(dafnyValue.dtor_nonSensitive().dtor_value()));
+    }
+    if (dafnyValue.dtor_constructors().is_Some()) {
+      nativeBuilder.constructors(ToNative.ConstructorList(dafnyValue.dtor_constructors().dtor_value()));
+    }
+    return nativeBuilder.build();
+  }
+
+  public static BatchWriteItemOutputTransformOutput BatchWriteItemOutputTransformOutput(
+      Dafny.Aws.Cryptography.DynamoDbEncryption.Types.BatchWriteItemOutputTransformOutput dafnyValue) {
+    BatchWriteItemOutputTransformOutput.Builder nativeBuilder = BatchWriteItemOutputTransformOutput.builder();
+    nativeBuilder.transformedOutput(Dafny.Com.Amazonaws.Dynamodb.ToNative.BatchWriteItemOutput(dafnyValue.dtor_transformedOutput()));
+    return nativeBuilder.build();
+  }
+
+  public static ScanOutputTransformOutput ScanOutputTransformOutput(
+      Dafny.Aws.Cryptography.DynamoDbEncryption.Types.ScanOutputTransformOutput dafnyValue) {
+    ScanOutputTransformOutput.Builder nativeBuilder = ScanOutputTransformOutput.builder();
+    nativeBuilder.transformedOutput(Dafny.Com.Amazonaws.Dynamodb.ToNative.ScanOutput(dafnyValue.dtor_transformedOutput()));
     return nativeBuilder.build();
   }
 
@@ -359,25 +571,115 @@ public class ToNative {
     return nativeBuilder.build();
   }
 
-  public static ExecuteStatementOutputTransformInput ExecuteStatementOutputTransformInput(
-      Dafny.Aws.Cryptography.DynamoDbEncryption.Types.ExecuteStatementOutputTransformInput dafnyValue) {
-    ExecuteStatementOutputTransformInput.Builder nativeBuilder = ExecuteStatementOutputTransformInput.builder();
-    nativeBuilder.sdkOutput(Dafny.Com.Amazonaws.Dynamodb.ToNative.ExecuteStatementOutput(dafnyValue.dtor_sdkOutput()));
-    nativeBuilder.originalInput(Dafny.Com.Amazonaws.Dynamodb.ToNative.ExecuteStatementInput(dafnyValue.dtor_originalInput()));
+  public static UpdateItemOutputTransformInput UpdateItemOutputTransformInput(
+      Dafny.Aws.Cryptography.DynamoDbEncryption.Types.UpdateItemOutputTransformInput dafnyValue) {
+    UpdateItemOutputTransformInput.Builder nativeBuilder = UpdateItemOutputTransformInput.builder();
+    nativeBuilder.sdkOutput(Dafny.Com.Amazonaws.Dynamodb.ToNative.UpdateItemOutput(dafnyValue.dtor_sdkOutput()));
+    nativeBuilder.originalInput(Dafny.Com.Amazonaws.Dynamodb.ToNative.UpdateItemInput(dafnyValue.dtor_originalInput()));
     return nativeBuilder.build();
   }
 
-  public static ScanOutputTransformOutput ScanOutputTransformOutput(
-      Dafny.Aws.Cryptography.DynamoDbEncryption.Types.ScanOutputTransformOutput dafnyValue) {
-    ScanOutputTransformOutput.Builder nativeBuilder = ScanOutputTransformOutput.builder();
-    nativeBuilder.transformedOutput(Dafny.Com.Amazonaws.Dynamodb.ToNative.ScanOutput(dafnyValue.dtor_transformedOutput()));
+  public static UpdateTableInputTransformOutput UpdateTableInputTransformOutput(
+      Dafny.Aws.Cryptography.DynamoDbEncryption.Types.UpdateTableInputTransformOutput dafnyValue) {
+    UpdateTableInputTransformOutput.Builder nativeBuilder = UpdateTableInputTransformOutput.builder();
+    nativeBuilder.transformedInput(Dafny.Com.Amazonaws.Dynamodb.ToNative.UpdateTableInput(dafnyValue.dtor_transformedInput()));
     return nativeBuilder.build();
   }
 
-  public static UpdateItemInputTransformInput UpdateItemInputTransformInput(
-      Dafny.Aws.Cryptography.DynamoDbEncryption.Types.UpdateItemInputTransformInput dafnyValue) {
-    UpdateItemInputTransformInput.Builder nativeBuilder = UpdateItemInputTransformInput.builder();
-    nativeBuilder.sdkInput(Dafny.Com.Amazonaws.Dynamodb.ToNative.UpdateItemInput(dafnyValue.dtor_sdkInput()));
+  public static QueryInputTransformInput QueryInputTransformInput(
+      Dafny.Aws.Cryptography.DynamoDbEncryption.Types.QueryInputTransformInput dafnyValue) {
+    QueryInputTransformInput.Builder nativeBuilder = QueryInputTransformInput.builder();
+    nativeBuilder.sdkInput(Dafny.Com.Amazonaws.Dynamodb.ToNative.QueryInput(dafnyValue.dtor_sdkInput()));
+    return nativeBuilder.build();
+  }
+
+  public static PutItemOutputTransformInput PutItemOutputTransformInput(
+      Dafny.Aws.Cryptography.DynamoDbEncryption.Types.PutItemOutputTransformInput dafnyValue) {
+    PutItemOutputTransformInput.Builder nativeBuilder = PutItemOutputTransformInput.builder();
+    nativeBuilder.sdkOutput(Dafny.Com.Amazonaws.Dynamodb.ToNative.PutItemOutput(dafnyValue.dtor_sdkOutput()));
+    nativeBuilder.originalInput(Dafny.Com.Amazonaws.Dynamodb.ToNative.PutItemInput(dafnyValue.dtor_originalInput()));
+    return nativeBuilder.build();
+  }
+
+  public static TransactGetItemsOutputTransformInput TransactGetItemsOutputTransformInput(
+      Dafny.Aws.Cryptography.DynamoDbEncryption.Types.TransactGetItemsOutputTransformInput dafnyValue) {
+    TransactGetItemsOutputTransformInput.Builder nativeBuilder = TransactGetItemsOutputTransformInput.builder();
+    nativeBuilder.sdkOutput(Dafny.Com.Amazonaws.Dynamodb.ToNative.TransactGetItemsOutput(dafnyValue.dtor_sdkOutput()));
+    nativeBuilder.originalInput(Dafny.Com.Amazonaws.Dynamodb.ToNative.TransactGetItemsInput(dafnyValue.dtor_originalInput()));
+    return nativeBuilder.build();
+  }
+
+  public static BatchWriteItemOutputTransformInput BatchWriteItemOutputTransformInput(
+      Dafny.Aws.Cryptography.DynamoDbEncryption.Types.BatchWriteItemOutputTransformInput dafnyValue) {
+    BatchWriteItemOutputTransformInput.Builder nativeBuilder = BatchWriteItemOutputTransformInput.builder();
+    nativeBuilder.sdkOutput(Dafny.Com.Amazonaws.Dynamodb.ToNative.BatchWriteItemOutput(dafnyValue.dtor_sdkOutput()));
+    nativeBuilder.originalInput(Dafny.Com.Amazonaws.Dynamodb.ToNative.BatchWriteItemInput(dafnyValue.dtor_originalInput()));
+    return nativeBuilder.build();
+  }
+
+  public static ScanInputTransformOutput ScanInputTransformOutput(
+      Dafny.Aws.Cryptography.DynamoDbEncryption.Types.ScanInputTransformOutput dafnyValue) {
+    ScanInputTransformOutput.Builder nativeBuilder = ScanInputTransformOutput.builder();
+    nativeBuilder.transformedInput(Dafny.Com.Amazonaws.Dynamodb.ToNative.ScanInput(dafnyValue.dtor_transformedInput()));
+    return nativeBuilder.build();
+  }
+
+  public static CreateTableOutputTransformInput CreateTableOutputTransformInput(
+      Dafny.Aws.Cryptography.DynamoDbEncryption.Types.CreateTableOutputTransformInput dafnyValue) {
+    CreateTableOutputTransformInput.Builder nativeBuilder = CreateTableOutputTransformInput.builder();
+    nativeBuilder.sdkOutput(Dafny.Com.Amazonaws.Dynamodb.ToNative.CreateTableOutput(dafnyValue.dtor_sdkOutput()));
+    nativeBuilder.originalInput(Dafny.Com.Amazonaws.Dynamodb.ToNative.CreateTableInput(dafnyValue.dtor_originalInput()));
+    return nativeBuilder.build();
+  }
+
+  public static ExecuteTransactionOutputTransformInput ExecuteTransactionOutputTransformInput(
+      Dafny.Aws.Cryptography.DynamoDbEncryption.Types.ExecuteTransactionOutputTransformInput dafnyValue) {
+    ExecuteTransactionOutputTransformInput.Builder nativeBuilder = ExecuteTransactionOutputTransformInput.builder();
+    nativeBuilder.sdkOutput(Dafny.Com.Amazonaws.Dynamodb.ToNative.ExecuteTransactionOutput(dafnyValue.dtor_sdkOutput()));
+    nativeBuilder.originalInput(Dafny.Com.Amazonaws.Dynamodb.ToNative.ExecuteTransactionInput(dafnyValue.dtor_originalInput()));
+    return nativeBuilder.build();
+  }
+
+  public static DescribeTableOutputTransformInput DescribeTableOutputTransformInput(
+      Dafny.Aws.Cryptography.DynamoDbEncryption.Types.DescribeTableOutputTransformInput dafnyValue) {
+    DescribeTableOutputTransformInput.Builder nativeBuilder = DescribeTableOutputTransformInput.builder();
+    nativeBuilder.sdkOutput(Dafny.Com.Amazonaws.Dynamodb.ToNative.DescribeTableOutput(dafnyValue.dtor_sdkOutput()));
+    nativeBuilder.originalInput(Dafny.Com.Amazonaws.Dynamodb.ToNative.DescribeTableInput(dafnyValue.dtor_originalInput()));
+    return nativeBuilder.build();
+  }
+
+  public static BatchWriteItemInputTransformInput BatchWriteItemInputTransformInput(
+      Dafny.Aws.Cryptography.DynamoDbEncryption.Types.BatchWriteItemInputTransformInput dafnyValue) {
+    BatchWriteItemInputTransformInput.Builder nativeBuilder = BatchWriteItemInputTransformInput.builder();
+    nativeBuilder.sdkInput(Dafny.Com.Amazonaws.Dynamodb.ToNative.BatchWriteItemInput(dafnyValue.dtor_sdkInput()));
+    return nativeBuilder.build();
+  }
+
+  public static DescribeTableInputTransformOutput DescribeTableInputTransformOutput(
+      Dafny.Aws.Cryptography.DynamoDbEncryption.Types.DescribeTableInputTransformOutput dafnyValue) {
+    DescribeTableInputTransformOutput.Builder nativeBuilder = DescribeTableInputTransformOutput.builder();
+    nativeBuilder.transformedInput(Dafny.Com.Amazonaws.Dynamodb.ToNative.DescribeTableInput(dafnyValue.dtor_transformedInput()));
+    return nativeBuilder.build();
+  }
+
+  public static ExecuteStatementInputTransformOutput ExecuteStatementInputTransformOutput(
+      Dafny.Aws.Cryptography.DynamoDbEncryption.Types.ExecuteStatementInputTransformOutput dafnyValue) {
+    ExecuteStatementInputTransformOutput.Builder nativeBuilder = ExecuteStatementInputTransformOutput.builder();
+    nativeBuilder.transformedInput(Dafny.Com.Amazonaws.Dynamodb.ToNative.ExecuteStatementInput(dafnyValue.dtor_transformedInput()));
+    return nativeBuilder.build();
+  }
+
+  public static BatchGetItemOutputTransformOutput BatchGetItemOutputTransformOutput(
+      Dafny.Aws.Cryptography.DynamoDbEncryption.Types.BatchGetItemOutputTransformOutput dafnyValue) {
+    BatchGetItemOutputTransformOutput.Builder nativeBuilder = BatchGetItemOutputTransformOutput.builder();
+    nativeBuilder.transformedOutput(Dafny.Com.Amazonaws.Dynamodb.ToNative.BatchGetItemOutput(dafnyValue.dtor_transformedOutput()));
+    return nativeBuilder.build();
+  }
+
+  public static CreateTableInputTransformOutput CreateTableInputTransformOutput(
+      Dafny.Aws.Cryptography.DynamoDbEncryption.Types.CreateTableInputTransformOutput dafnyValue) {
+    CreateTableInputTransformOutput.Builder nativeBuilder = CreateTableInputTransformOutput.builder();
+    nativeBuilder.transformedInput(Dafny.Com.Amazonaws.Dynamodb.ToNative.CreateTableInput(dafnyValue.dtor_transformedInput()));
     return nativeBuilder.build();
   }
 
@@ -385,27 +687,6 @@ public class ToNative {
       Dafny.Aws.Cryptography.DynamoDbEncryption.Types.BatchWriteItemInputTransformOutput dafnyValue) {
     BatchWriteItemInputTransformOutput.Builder nativeBuilder = BatchWriteItemInputTransformOutput.builder();
     nativeBuilder.transformedInput(Dafny.Com.Amazonaws.Dynamodb.ToNative.BatchWriteItemInput(dafnyValue.dtor_transformedInput()));
-    return nativeBuilder.build();
-  }
-
-  public static TransactWriteItemsOutputTransformOutput TransactWriteItemsOutputTransformOutput(
-      Dafny.Aws.Cryptography.DynamoDbEncryption.Types.TransactWriteItemsOutputTransformOutput dafnyValue) {
-    TransactWriteItemsOutputTransformOutput.Builder nativeBuilder = TransactWriteItemsOutputTransformOutput.builder();
-    nativeBuilder.transformedOutput(Dafny.Com.Amazonaws.Dynamodb.ToNative.TransactWriteItemsOutput(dafnyValue.dtor_transformedOutput()));
-    return nativeBuilder.build();
-  }
-
-  public static TransactGetItemsInputTransformInput TransactGetItemsInputTransformInput(
-      Dafny.Aws.Cryptography.DynamoDbEncryption.Types.TransactGetItemsInputTransformInput dafnyValue) {
-    TransactGetItemsInputTransformInput.Builder nativeBuilder = TransactGetItemsInputTransformInput.builder();
-    nativeBuilder.sdkInput(Dafny.Com.Amazonaws.Dynamodb.ToNative.TransactGetItemsInput(dafnyValue.dtor_sdkInput()));
-    return nativeBuilder.build();
-  }
-
-  public static DynamoDbEncryptionConfig DynamoDbEncryptionConfig(
-      Dafny.Aws.Cryptography.DynamoDbEncryption.Types.DynamoDbEncryptionConfig dafnyValue) {
-    DynamoDbEncryptionConfig.Builder nativeBuilder = DynamoDbEncryptionConfig.builder();
-    nativeBuilder.tableEncryptionConfigs(ToNative.DynamoDbTableEncryptionConfigs(dafnyValue.dtor_tableEncryptionConfigs()));
     return nativeBuilder.build();
   }
 
@@ -423,99 +704,75 @@ public class ToNative {
     return nativeBuilder.build();
   }
 
-  public static TransactGetItemsOutputTransformInput TransactGetItemsOutputTransformInput(
-      Dafny.Aws.Cryptography.DynamoDbEncryption.Types.TransactGetItemsOutputTransformInput dafnyValue) {
-    TransactGetItemsOutputTransformInput.Builder nativeBuilder = TransactGetItemsOutputTransformInput.builder();
-    nativeBuilder.sdkOutput(Dafny.Com.Amazonaws.Dynamodb.ToNative.TransactGetItemsOutput(dafnyValue.dtor_sdkOutput()));
-    nativeBuilder.originalInput(Dafny.Com.Amazonaws.Dynamodb.ToNative.TransactGetItemsInput(dafnyValue.dtor_originalInput()));
+  public static ExecuteStatementOutputTransformInput ExecuteStatementOutputTransformInput(
+      Dafny.Aws.Cryptography.DynamoDbEncryption.Types.ExecuteStatementOutputTransformInput dafnyValue) {
+    ExecuteStatementOutputTransformInput.Builder nativeBuilder = ExecuteStatementOutputTransformInput.builder();
+    nativeBuilder.sdkOutput(Dafny.Com.Amazonaws.Dynamodb.ToNative.ExecuteStatementOutput(dafnyValue.dtor_sdkOutput()));
+    nativeBuilder.originalInput(Dafny.Com.Amazonaws.Dynamodb.ToNative.ExecuteStatementInput(dafnyValue.dtor_originalInput()));
     return nativeBuilder.build();
   }
 
-  public static UpdateItemOutputTransformInput UpdateItemOutputTransformInput(
-      Dafny.Aws.Cryptography.DynamoDbEncryption.Types.UpdateItemOutputTransformInput dafnyValue) {
-    UpdateItemOutputTransformInput.Builder nativeBuilder = UpdateItemOutputTransformInput.builder();
-    nativeBuilder.sdkOutput(Dafny.Com.Amazonaws.Dynamodb.ToNative.UpdateItemOutput(dafnyValue.dtor_sdkOutput()));
-    nativeBuilder.originalInput(Dafny.Com.Amazonaws.Dynamodb.ToNative.UpdateItemInput(dafnyValue.dtor_originalInput()));
+  public static TransactWriteItemsOutputTransformOutput TransactWriteItemsOutputTransformOutput(
+      Dafny.Aws.Cryptography.DynamoDbEncryption.Types.TransactWriteItemsOutputTransformOutput dafnyValue) {
+    TransactWriteItemsOutputTransformOutput.Builder nativeBuilder = TransactWriteItemsOutputTransformOutput.builder();
+    nativeBuilder.transformedOutput(Dafny.Com.Amazonaws.Dynamodb.ToNative.TransactWriteItemsOutput(dafnyValue.dtor_transformedOutput()));
     return nativeBuilder.build();
   }
 
-  public static BatchWriteItemInputTransformInput BatchWriteItemInputTransformInput(
-      Dafny.Aws.Cryptography.DynamoDbEncryption.Types.BatchWriteItemInputTransformInput dafnyValue) {
-    BatchWriteItemInputTransformInput.Builder nativeBuilder = BatchWriteItemInputTransformInput.builder();
-    nativeBuilder.sdkInput(Dafny.Com.Amazonaws.Dynamodb.ToNative.BatchWriteItemInput(dafnyValue.dtor_sdkInput()));
-    return nativeBuilder.build();
+  public static List<VirtualField> VirtualFieldList(
+      DafnySequence<? extends Dafny.Aws.Cryptography.DynamoDbEncryption.Types.VirtualField> dafnyValue) {
+    return software.amazon.dafny.conversion.ToNative.Aggregate.GenericToList(
+        dafnyValue, 
+        software.amazon.cryptography.dynamoDbEncryption.ToNative::VirtualField);
   }
 
-  public static ScanInputTransformInput ScanInputTransformInput(
-      Dafny.Aws.Cryptography.DynamoDbEncryption.Types.ScanInputTransformInput dafnyValue) {
-    ScanInputTransformInput.Builder nativeBuilder = ScanInputTransformInput.builder();
-    nativeBuilder.sdkInput(Dafny.Com.Amazonaws.Dynamodb.ToNative.ScanInput(dafnyValue.dtor_sdkInput()));
-    return nativeBuilder.build();
+  public static List<StandardBeacon> StandardBeaconList(
+      DafnySequence<? extends Dafny.Aws.Cryptography.DynamoDbEncryption.Types.StandardBeacon> dafnyValue) {
+    return software.amazon.dafny.conversion.ToNative.Aggregate.GenericToList(
+        dafnyValue, 
+        software.amazon.cryptography.dynamoDbEncryption.ToNative::StandardBeacon);
   }
 
-  public static BatchWriteItemOutputTransformInput BatchWriteItemOutputTransformInput(
-      Dafny.Aws.Cryptography.DynamoDbEncryption.Types.BatchWriteItemOutputTransformInput dafnyValue) {
-    BatchWriteItemOutputTransformInput.Builder nativeBuilder = BatchWriteItemOutputTransformInput.builder();
-    nativeBuilder.sdkOutput(Dafny.Com.Amazonaws.Dynamodb.ToNative.BatchWriteItemOutput(dafnyValue.dtor_sdkOutput()));
-    nativeBuilder.originalInput(Dafny.Com.Amazonaws.Dynamodb.ToNative.BatchWriteItemInput(dafnyValue.dtor_originalInput()));
-    return nativeBuilder.build();
+  public static List<NonSensitivePart> NonSensitivePartsList(
+      DafnySequence<? extends Dafny.Aws.Cryptography.DynamoDbEncryption.Types.NonSensitivePart> dafnyValue) {
+    return software.amazon.dafny.conversion.ToNative.Aggregate.GenericToList(
+        dafnyValue, 
+        software.amazon.cryptography.dynamoDbEncryption.ToNative::NonSensitivePart);
   }
 
-  public static QueryInputTransformInput QueryInputTransformInput(
-      Dafny.Aws.Cryptography.DynamoDbEncryption.Types.QueryInputTransformInput dafnyValue) {
-    QueryInputTransformInput.Builder nativeBuilder = QueryInputTransformInput.builder();
-    nativeBuilder.sdkInput(Dafny.Com.Amazonaws.Dynamodb.ToNative.QueryInput(dafnyValue.dtor_sdkInput()));
-    return nativeBuilder.build();
+  public static List<SensitivePart> SensitivePartsList(
+      DafnySequence<? extends Dafny.Aws.Cryptography.DynamoDbEncryption.Types.SensitivePart> dafnyValue) {
+    return software.amazon.dafny.conversion.ToNative.Aggregate.GenericToList(
+        dafnyValue, 
+        software.amazon.cryptography.dynamoDbEncryption.ToNative::SensitivePart);
   }
 
-  public static TransactGetItemsInputTransformOutput TransactGetItemsInputTransformOutput(
-      Dafny.Aws.Cryptography.DynamoDbEncryption.Types.TransactGetItemsInputTransformOutput dafnyValue) {
-    TransactGetItemsInputTransformOutput.Builder nativeBuilder = TransactGetItemsInputTransformOutput.builder();
-    nativeBuilder.transformedInput(Dafny.Com.Amazonaws.Dynamodb.ToNative.TransactGetItemsInput(dafnyValue.dtor_transformedInput()));
-    return nativeBuilder.build();
+  public static List<CompoundBeacon> CompoundBeaconList(
+      DafnySequence<? extends Dafny.Aws.Cryptography.DynamoDbEncryption.Types.CompoundBeacon> dafnyValue) {
+    return software.amazon.dafny.conversion.ToNative.Aggregate.GenericToList(
+        dafnyValue, 
+        software.amazon.cryptography.dynamoDbEncryption.ToNative::CompoundBeacon);
   }
 
-  public static TransactGetItemsOutputTransformOutput TransactGetItemsOutputTransformOutput(
-      Dafny.Aws.Cryptography.DynamoDbEncryption.Types.TransactGetItemsOutputTransformOutput dafnyValue) {
-    TransactGetItemsOutputTransformOutput.Builder nativeBuilder = TransactGetItemsOutputTransformOutput.builder();
-    nativeBuilder.transformedOutput(Dafny.Com.Amazonaws.Dynamodb.ToNative.TransactGetItemsOutput(dafnyValue.dtor_transformedOutput()));
-    return nativeBuilder.build();
+  public static List<Constructor> ConstructorList(
+      DafnySequence<? extends Dafny.Aws.Cryptography.DynamoDbEncryption.Types.Constructor> dafnyValue) {
+    return software.amazon.dafny.conversion.ToNative.Aggregate.GenericToList(
+        dafnyValue, 
+        software.amazon.cryptography.dynamoDbEncryption.ToNative::Constructor);
   }
 
-  public static ExecuteStatementInputTransformInput ExecuteStatementInputTransformInput(
-      Dafny.Aws.Cryptography.DynamoDbEncryption.Types.ExecuteStatementInputTransformInput dafnyValue) {
-    ExecuteStatementInputTransformInput.Builder nativeBuilder = ExecuteStatementInputTransformInput.builder();
-    nativeBuilder.sdkInput(Dafny.Com.Amazonaws.Dynamodb.ToNative.ExecuteStatementInput(dafnyValue.dtor_sdkInput()));
-    return nativeBuilder.build();
+  public static List<BeaconVersion> BeaconVersionList(
+      DafnySequence<? extends Dafny.Aws.Cryptography.DynamoDbEncryption.Types.BeaconVersion> dafnyValue) {
+    return software.amazon.dafny.conversion.ToNative.Aggregate.GenericToList(
+        dafnyValue, 
+        software.amazon.cryptography.dynamoDbEncryption.ToNative::BeaconVersion);
   }
 
-  public static ExecuteTransactionInputTransformOutput ExecuteTransactionInputTransformOutput(
-      Dafny.Aws.Cryptography.DynamoDbEncryption.Types.ExecuteTransactionInputTransformOutput dafnyValue) {
-    ExecuteTransactionInputTransformOutput.Builder nativeBuilder = ExecuteTransactionInputTransformOutput.builder();
-    nativeBuilder.transformedInput(Dafny.Com.Amazonaws.Dynamodb.ToNative.ExecuteTransactionInput(dafnyValue.dtor_transformedInput()));
-    return nativeBuilder.build();
-  }
-
-  public static UpdateItemInputTransformOutput UpdateItemInputTransformOutput(
-      Dafny.Aws.Cryptography.DynamoDbEncryption.Types.UpdateItemInputTransformOutput dafnyValue) {
-    UpdateItemInputTransformOutput.Builder nativeBuilder = UpdateItemInputTransformOutput.builder();
-    nativeBuilder.transformedInput(Dafny.Com.Amazonaws.Dynamodb.ToNative.UpdateItemInput(dafnyValue.dtor_transformedInput()));
-    return nativeBuilder.build();
-  }
-
-  public static ExecuteTransactionOutputTransformInput ExecuteTransactionOutputTransformInput(
-      Dafny.Aws.Cryptography.DynamoDbEncryption.Types.ExecuteTransactionOutputTransformInput dafnyValue) {
-    ExecuteTransactionOutputTransformInput.Builder nativeBuilder = ExecuteTransactionOutputTransformInput.builder();
-    nativeBuilder.sdkOutput(Dafny.Com.Amazonaws.Dynamodb.ToNative.ExecuteTransactionOutput(dafnyValue.dtor_sdkOutput()));
-    nativeBuilder.originalInput(Dafny.Com.Amazonaws.Dynamodb.ToNative.ExecuteTransactionInput(dafnyValue.dtor_originalInput()));
-    return nativeBuilder.build();
-  }
-
-  public static ScanInputTransformOutput ScanInputTransformOutput(
-      Dafny.Aws.Cryptography.DynamoDbEncryption.Types.ScanInputTransformOutput dafnyValue) {
-    ScanInputTransformOutput.Builder nativeBuilder = ScanInputTransformOutput.builder();
-    nativeBuilder.transformedInput(Dafny.Com.Amazonaws.Dynamodb.ToNative.ScanInput(dafnyValue.dtor_transformedInput()));
-    return nativeBuilder.build();
+  public static List<ConstructorPart> ConstructorPartList(
+      DafnySequence<? extends Dafny.Aws.Cryptography.DynamoDbEncryption.Types.ConstructorPart> dafnyValue) {
+    return software.amazon.dafny.conversion.ToNative.Aggregate.GenericToList(
+        dafnyValue, 
+        software.amazon.cryptography.dynamoDbEncryption.ToNative::ConstructorPart);
   }
 
   public static Map<String, DynamoDbTableEncryptionConfig> DynamoDbTableEncryptionConfigs(
