DynamoDbEncryptionMiddlewareInternal/runtimes/java/src/main/smithy-generated/software/amazon/cryptography/dynamoDbEncryption/model/NonSensitivePart.java
@@ -1,0 +1,90 @@
+// Copyright Amazon.com Inc. or its affiliates. All Rights Reserved.
+// SPDX-License-Identifier: Apache-2.0
+// Do not modify this file. This file is machine generated, and any changes to it will be overwritten.
+package software.amazon.cryptography.dynamoDbEncryption.model;
+
+import java.util.Objects;
+
+public class NonSensitivePart {
+  private final String name;
+
+  private final String loc;
+
+  protected NonSensitivePart(BuilderImpl builder) {
+    this.name = builder.name();
+    this.loc = builder.loc();
+  }
+
+  public String name() {
+    return this.name;
+  }
+
+  public String loc() {
+    return this.loc;
+  }
+
+  public Builder toBuilder() {
+    return new BuilderImpl(this);
+  }
+
+  public static Builder builder() {
+    return new BuilderImpl();
+  }
+
+  public interface Builder {
+    Builder name(String name);
+
+    String name();
+
+    Builder loc(String loc);
+
+    String loc();
+
+    NonSensitivePart build();
+  }
+
+  static class BuilderImpl implements Builder {
+    protected String name;
+
+    protected String loc;
+
+    protected BuilderImpl() {
+    }
+
+    protected BuilderImpl(NonSensitivePart model) {
+      this.name = model.name();
+      this.loc = model.loc();
+    }
+
+    public Builder name(String name) {
+      this.name = name;
+      return this;
+    }
+
+    public String name() {
+      return this.name;
+    }
+
+    public Builder loc(String loc) {
+      this.loc = loc;
+      return this;
+    }
+
+    public String loc() {
+      return this.loc;
+    }
+
+    public NonSensitivePart build() {
+      if (Objects.isNull(this.name()))  {
+        throw new IllegalArgumentException("Missing value for required field `name`");
+      }
+      if (Objects.isNull(this.loc()))  {
+        throw new IllegalArgumentException("Missing value for required field `loc`");
+      }
+      if (Objects.nonNull(this.loc()) && this.loc().length() < 1) {
+        throw new IllegalArgumentException("The size of `loc` must be greater than or equal to 1");
+      }
+      return new NonSensitivePart(this);
+    }
+  }
+}
